reflex/coq/PruneFacts.v
@@ -1,12 +1,17 @@
 Require Import Reflex.
 Require Import ReflexBase.
 Require Import ReflexHVec.
+Require Import ReflexVec.
 Require Import ReflexFin.
 Require Import ReflexDenoted.
 Require Import ReflexIO.
 Require Import List.
 
+Require Import NIExists.
+Require Import Ynot.
+
 Require Import Coq.Logic.Eqdep.
+Require Import Sumbool.
 
 Section Prune.
 
@@ -17,19 +22,983 @@ Variable COMPTDEC : forall (x y : COMPT), decide (x = y).
 Variable COMPS    : COMPT -> compd.
 Variable IENVD    : vcdesc COMPT.
 Variable KSTD     : vcdesc COMPT.
-Variable INIT : init_prog PAYD COMPT COMPS KSTD IENVD.
-Variable HANDLERS : handlers PAYD COMPT COMPS KSTD.
+Definition ReachInter := NIExists.ReachInter PAYD COMPT COMPTDEC COMPS KSTD.
 Definition comp := comp COMPT COMPS.
-Definition Reach := Reflex.Reach PAYD COMPT COMPTDEC COMPS KSTD IENVD INIT.
-Definition ValidExchange := ValidExchange PAYD COMPT COMPTDEC COMPS KSTD HANDLERS.
 Definition KTrace := KTrace PAYD COMPT COMPS.
 Definition KAction := KAction PAYD COMPT COMPS.
 Definition kstate := kstate PAYD COMPT COMPS KSTD.
 Definition ktr := ktr PAYD COMPT COMPS KSTD.
 Definition Nop := Reflex.Nop PAYD COMPT COMPS KSTD.
+Definition Seq := Reflex.Seq PAYD COMPT COMPS KSTD.
+Definition Send := Reflex.Send PAYD COMPT COMPS KSTD.
+Definition StUpd := Reflex.StUpd PAYD COMPT COMPS KSTD.
+Definition Spawn := Reflex.Spawn PAYD COMPT COMPS KSTD.
+Definition Call := Reflex.Call PAYD COMPT COMPS KSTD.
+Definition Ite := Reflex.Ite PAYD COMPT COMPS KSTD.
+Definition CompLkup := Reflex.CompLkup PAYD COMPT COMPS KSTD.
+Definition hdlr_term := Reflex.hdlr_term PAYD COMPT COMPS KSTD.
+Definition base_term := Reflex.base_term COMPT.
+Definition match_comp := Reflex.match_comp COMPT COMPTDEC COMPS.
+Definition cmd := Reflex.cmd PAYD COMPT COMPS KSTD.
 
-Require Import NIExists.
-Require Import Ynot.
+Definition locals_eq (envd:vcdesc COMPT)
+  (env1 env2 : sdenote_vcdesc COMPT COMPS envd)
+  (lblr : fin (projT1 envd) -> bool) :=  
+  shvec_erase _ lblr _ env1 = shvec_erase _ lblr _ env2.
+
+Definition ve_st c m envd cmd i s :=
+    hdlr_state_run_cmd PAYD COMPT COMPTDEC COMPS KSTD c m
+    envd s cmd i.
+
+Definition base_term_ok_high envd d (t:base_term envd d) llblr :=
+  match t with
+  | SLit _ => true
+  | NLit _ => true
+  | Var i  => llblr i
+  | _      => false
+  end.
+
+Fixpoint hdlr_term_ok_high ct mt envd c (t:hdlr_term ct mt envd c) vlblr llblr :=
+  match t with
+  | Base _ b    => base_term_ok_high _ _ b llblr
+  | MVar _      => true
+  | StVar i     => vlblr i
+  | CComp       => true
+  | CConf _ _ t => hdlr_term_ok_high _ _ _ _ t vlblr llblr
+  end.
+
+Fixpoint hdlr_expr_ok_high ct mt envd c
+  (e:expr COMPT (hdlr_term ct mt) envd c) vlblr llblr :=
+  match e with
+  | Term _ t => hdlr_term_ok_high _ _ _ _ t vlblr llblr
+  | UnOp _ _ _ e' => hdlr_expr_ok_high _ _ _ _ e' vlblr llblr
+  | BinOp _ _ _ _ e1 e2 => andb (hdlr_expr_ok_high _ _ _ _ e1 vlblr llblr)
+    (hdlr_expr_ok_high _ _ _ _ e2 vlblr llblr)
+  end.
+
+Definition hdlr_oexpr_ok_high ct mt envd c
+  (oe:option (expr COMPT (hdlr_term ct mt) envd c))
+  vlblr llblr :=
+  match oe with
+  | Some e => hdlr_expr_ok_high ct mt envd c e vlblr llblr
+  | None => true
+  end.
+
+Definition expr_list_ok_high ct mt envd c
+  (es:list (expr COMPT (hdlr_term ct mt) envd c)) vlblr llblr :=
+  fold_right (fun e => andb
+    (hdlr_expr_ok_high ct mt envd c e vlblr llblr)) true es.
+
+Fixpoint pl_expr_ok_high ct mt envd n vd
+  (ple:payload_expr' COMPT (hdlr_term ct mt) envd n vd) vlblr llblr :=
+  match n as _n return
+    forall (_vd:vdesc' _n) (ple:payload_expr' COMPT (hdlr_term ct mt) envd _n _vd), _
+  with
+  | O => fun _ _ => true
+  | S n' => fun vd =>
+    match vd as _vd return
+      payload_expr' COMPT (hdlr_term ct mt) envd (S n') _vd -> _
+    with
+    | (vd0, vd') =>
+      fun ple =>
+        andb (hdlr_expr_ok_high ct mt envd _ (fst ple) vlblr llblr)
+          (pl_expr_ok_high ct mt envd n' _ (snd ple) vlblr llblr)
+    end
+  end vd ple.
+
+Fixpoint pl_oexpr_ok_high ct mt envd n vd
+  (ple:payload_oexpr' COMPT (hdlr_term ct mt) envd n vd) vlblr llblr :=
+  match n as _n return
+    forall (_vd:vdesc' _n) (ple:payload_oexpr' COMPT (hdlr_term ct mt) envd _n _vd), _
+  with
+  | O => fun _ _ => true
+  | S n' => fun vd =>
+    match vd as _vd return
+      payload_oexpr' COMPT (hdlr_term ct mt) envd (S n') _vd -> _
+    with
+    | (vd0, vd') =>
+      fun ple =>
+        andb (hdlr_oexpr_ok_high ct mt envd _ (fst ple) vlblr llblr)
+          (pl_oexpr_ok_high ct mt envd n' _ (snd ple) vlblr llblr)
+    end
+  end vd ple.
+
+Fixpoint get_writes envd term (cmd:cmd term envd) :=
+  match cmd in Reflex.cmd _ _ _ _ _ _envd return
+    fin (projT1 _envd) -> bool
+  with
+  | Reflex.Seq _ cmd1 cmd2 =>
+    fun i => andb (get_writes _ _ cmd1 i)
+      (get_writes _ _ cmd2 i)
+  | Reflex.Ite _ _ cmd1 cmd2 =>
+    fun i => andb (get_writes _ _ cmd1 i)
+      (get_writes _ _ cmd2 i)
+  | Reflex.Spawn _ _ _ i' _ =>
+    fun i => if fin_eq_dec i i' then false else true
+  | Reflex.Call _ _ _ i' _ =>
+    fun i => if fin_eq_dec i i' then false else true
+  | Reflex.CompLkup _ _ i' _ cmd1 cmd2 =>
+    fun i =>
+      if fin_eq_dec i i'
+      then false
+      else andb (get_writes _ _ cmd1 i)
+        (get_writes _ _ cmd2 i)
+  | _ =>
+    fun _ => true
+  end.
+
+Definition cp_incl cp1 cp2 :=
+  forall c, implb (match_comp cp1 c)
+    (match_comp cp2 c) = true.
+
+Definition elt_incl d oelt1 oelt2 :=
+  forall elt,
+    implb (elt_match d elt oelt1)
+    (elt_match d elt oelt2) = true.
+
+Lemma desc_2 : forall (d:desc),
+  ex (fun s1:s[[d]] => ex (fun s2:s[[d]] => s1 <> s2)).
+Proof.
+  destruct d.
+    exists FALSE. exists TRUE. discriminate.
+    Local Transparent str_of_string.
+    exists (str_of_string ""). exists (str_of_string "a").
+    discriminate.
+    exists FALSE. exists TRUE. discriminate.
+Qed.
+
+Lemma desc_neq : forall (d:desc) (s:s[[d]]),
+  exists s', s <> s'.
+Proof.
+  intros d s. pose proof (desc_2 d).
+  destruct H. destruct H.
+  destruct d.
+    destruct (num_eq s x).
+      exists x0. congruence.
+      exists x. auto.
+
+    destruct (str_eq s x).
+      exists x0. congruence.
+      exists x. auto.
+
+    destruct (fd_eq s x).
+      exists x0. congruence.
+      exists x. auto.
+Qed.
+
+Lemma elt_incl_iff : forall d oelt1 oelt2,
+  elt_incl d oelt1 oelt2 <->
+  oelt2 = None \/ oelt1 = oelt2.
+Proof.
+  intros d oelt1 oelt2.
+  split.
+    intro Hincl. destruct oelt2.
+      right. unfold elt_incl, elt_match in Hincl. simpl in Hincl.
+      destruct oelt1.
+        destruct d; specialize (Hincl s0); simpl in *;
+          repeat match goal with
+                 | [ _ : context[ if ?e then _ else _ ] |- _ ]
+                   => destruct e
+                 end; try solve [subst s; auto | discriminate |
+                   specialize (n (Logic.eq_refl _)); contradiction].
+
+        pose proof (desc_neq d s). destruct H.
+        specialize (Hincl x). destruct d;
+        match goal with
+        | [ _ : context[ if ?e then _ else _ ] |- _ ]
+          => destruct e
+        end; try discriminate; try contradiction.
+
+      left. auto.
+
+    intro H. destruct H.
+      subst oelt2. unfold elt_incl. simpl.
+      intros. unfold implb. destruct (elt_match d elt oelt1); auto.
+
+      subst oelt1. unfold elt_incl. simpl. intros.
+      unfold implb. destruct (elt_match d elt oelt2); auto.
+Qed.
+
+Definition elt_incl_dec d oelt1 oelt2 :
+  decide (elt_incl d oelt1 oelt2).
+Proof.
+  destruct oelt2.
+    destruct oelt1.
+    destruct d.
+      destruct (num_eq s0 s);
+        [left; subst s; apply elt_incl_iff; auto
+          | right; intro H; apply elt_incl_iff in H;
+            destruct H; try inversion H; contradiction].
+      destruct (str_eq s0 s);
+        [left; subst s; apply elt_incl_iff; auto
+          | right; intro H; apply elt_incl_iff in H;
+            destruct H; try inversion H; contradiction].
+      destruct (fd_eq s0 s);
+        [left; subst s; apply elt_incl_iff; auto
+          | right; intro H; apply elt_incl_iff in H;
+            destruct H; try inversion H; contradiction].
+
+    right. intro H. apply elt_incl_iff in H. destruct H; discriminate.
+
+    left. apply elt_incl_iff. auto.
+Qed.
+
+Definition default_desc (d:desc) : s[[d]] :=
+match d with
+| num_d => FALSE
+| str_d => nil
+| fd_d => devnull
+end.
+
+Definition default_desc_match (d:desc) (oelt:sdenote_desc_conc_pat d)
+  : s[[d]] :=
+match oelt with
+| Some e => e
+| None => default_desc d
+end.
+
+Lemma default_desc_match_ok : forall d oelt,
+  elt_match d (default_desc_match d oelt) oelt = true.
+Proof.
+  intros d oelt.
+  destruct oelt; auto.
+  simpl. destruct d;
+  match goal with
+  |- context [ if ?e then _ else _ ]
+    => destruct e
+  end; auto.
+Qed.
+
+Definition non_match_vdesc n (vd:svec desc n) vdp :
+  sig (fun v:s[[vd]] => shvec_match vd sdenote_desc sdenote_desc_conc_pat elt_match v vdp = true).
+Proof.
+  induction n.
+    exact (exist _ tt (Logic.eq_refl _)).
+
+    destruct vd as [d vd']. destruct vdp as [od vdp']. simpl in *.
+    specialize (IHn vd' vdp'). destruct IHn.
+    refine (exist _ (default_desc_match d od, x) _).
+    rewrite default_desc_match_ok; auto.
+Qed.
+
+Definition cfgp_incl (cfgd:vdesc) cfgp1 cfgp2 :=
+  forall cfg, implb 
+    (shvec_match (projT2 cfgd)
+      sdenote_desc sdenote_desc_conc_pat elt_match
+      cfg cfgp1)
+    (shvec_match (projT2 cfgd)
+      sdenote_desc sdenote_desc_conc_pat elt_match
+      cfg cfgp2) = true.
+
+Definition cfgp_incl_dec (cfgd:vdesc) cfgp1 cfgp2 :
+  decide (cfgp_incl cfgd cfgp1 cfgp2).
+Proof.
+  destruct cfgd as [n cfgd]. unfold cfgp_incl.
+  induction n.
+    auto.
+
+    simpl in *. destruct cfgd as [? cfgd'].
+    destruct cfgp1 as [oelt1 cfgp1']. destruct cfgp2 as [oelt2 cfgp2'].
+    specialize (IHn cfgd' cfgp1' cfgp2').
+    destruct (elt_incl_dec d oelt1 oelt2).
+      destruct IHn.
+        left. intro cfg. destruct cfg as [elt cfg'].
+        specialize (e elt).
+        destruct (elt_match d elt oelt1).
+          destruct (elt_match d elt oelt2); try discriminate.
+          simpl. auto.
+          
+          auto.
+
+        right. intro.
+
+contradict n0. intro cfg.
+specialize (H (default_desc_match d oelt1, cfg)).
+specialize (e (default_desc_match d oelt1)). simpl in *.
+rewrite default_desc_match_ok in *. simpl in *.
+rewrite e in *. simpl in *. auto.
+
+right. intro. contradict n0.
+unfold elt_incl. intro elt.
+
+pose proof (non_match_vdesc n cfgd' cfgp1') as rest.
+destruct rest as [rest Hrest].
+specialize (H (elt, rest)). simpl in *. rewrite Hrest in H.
+simpl in *. destruct (elt_match d elt oelt1); auto.
+simpl in *. destruct (elt_match d elt oelt2); auto.
+Defined.
+
+Definition cp_incl_dec cp1 cp2 : decide (cp_incl cp1 cp2).
+Proof.
+  destruct cp1 as [ct1 cfg1]; destruct cp2 as [ct2 cfg2].
+  destruct (COMPTDEC ct1 ct2).
+    subst ct1. 
+    destruct (cfgp_incl_dec _ cfg1 cfg2).
+      left. unfold cp_incl, match_comp, Reflex.match_comp, match_comp_pf.
+      simpl. intro cp.
+      destruct (COMPTDEC (comp_type COMPT COMPS cp) ct2); auto. destruct e.
+      specialize (c (comp_conf _ _ cp)).
+      destruct (shvec_match
+              (projT2 (comp_conf_desc COMPT COMPS (comp_type COMPT COMPS cp)))
+              sdenote_desc sdenote_desc_conc_pat elt_match
+              (comp_conf COMPT COMPS cp) cfg1);
+      destruct (shvec_match
+              (projT2 (comp_conf_desc COMPT COMPS (comp_type COMPT COMPS cp)))
+              sdenote_desc sdenote_desc_conc_pat elt_match
+              (comp_conf COMPT COMPS cp) cfg2); auto.
+
+      right. intro. contradict n. intro cfg. unfold cp_incl in *.
+      specialize (H {|comp_type:=ct2; comp_fd:=devnull; comp_conf:=cfg|}).
+      unfold match_comp, Reflex.match_comp, match_comp_pf in *. simpl in *.
+      destruct (COMPTDEC ct2 ct2); auto.
+      rewrite UIP_refl with (p:=e) in *.
+      destruct (shvec_match (projT2 (comp_conf_desc COMPT COMPS ct2))
+                 sdenote_desc sdenote_desc_conc_pat
+                 elt_match cfg cfg1);
+      destruct (shvec_match (projT2 (comp_conf_desc COMPT COMPS ct2))
+                 sdenote_desc sdenote_desc_conc_pat
+                 elt_match cfg cfg2); auto.
+
+      right. intro.
+      pose proof (non_match_vdesc _ _ cfg1) as Hmatch.
+      destruct Hmatch as [v Hv].
+      specialize (H {|comp_type:=ct1;
+        comp_fd:=devnull;
+        comp_conf:=v|}).
+      unfold match_comp, Reflex.match_comp, match_comp_pf in *.
+      simpl in *. destruct (COMPTDEC ct1 ct2); try contradiction.
+      destruct (COMPTDEC ct1 ct1).
+      rewrite UIP_refl with (p:=e) in *. unfold elt_match in *.
+      rewrite Hv in *. discriminate.
+      contradict n1. auto.
+Qed.
+
+(*Definition high_cp_dec cp clblr :
+  decide (high_comp_pat COMPT COMPTDEC COMPS cp
+    (lblr_match_comp COMPT COMPTDEC COMPS clblr)).
+Proof.
+  induction clblr.
+    left. unfold high_comp_pat. intros. simpl. auto.
+
+    destruct IHclblr.
+      left. unfold high_comp_pat. intros c Hmatch.
+      specialize (h c Hmatch). unfold lblr_match_comp in *.
+      destruct clblr. simpl in *. auto. simpl in *.
+      rewrite h. auto.
+
+      destruct (cp_incl_dec cp a).
+        left. unfold high_comp_pat. intros comp Hmatch.
+        specialize (c comp). unfold match_comp, NIExists.match_comp in *. rewrite Hmatch in c.
+        simpl in *. unfold NIExists.match_comp. rewrite c. rewrite Bool.orb_true_r. auto.
+
+        right. intro. unfold high_comp_pat in *.
+      admit.
+Qed.*)
+
+(*Fixpoint get_candidate_pats clblr ct :
+  list (shvec sdenote_desc_conc_pat (projT2 (compd_conf (COMPS ct)))) :=
+  match clblr with
+  | nil => nil
+  | a::clblr' => 
+    match COMPTDEC ct (conc_pat_type _ COMPS a) with
+    | left EQ =>
+      match EQ in _ = _ct return
+        shvec sdenote_desc_conc_pat (projT2 (compd_conf (COMPS _ct))) -> _
+      with
+      | Logic.eq_refl => fun cfg0 =>
+        cfg0::get_candidate_pats clblr' ct
+      end (conc_pat_conf _ COMPS a)
+    | right _ => get_candidate_pats clblr' ct
+    end
+  end.
+
+Definition desc_val_eq {d:desc}
+  : forall (e1 e2:s[[d]]), decide (e1 = e2) :=
+  match d with
+  | num_d => num_eq
+  | str_d => str_eq
+  | fd_d  => fd_eq
+  end.
+
+Definition merge_desc_pats (d:desc) (o1 o2:option s[[d]])
+  : option s[[d]] :=
+  match o1 with
+  | Some e1 =>
+    match o2 with
+    | Some e2 => if desc_val_eq e1 e2
+                 then Some e1
+                 else None
+    | None    => None
+    end
+  | None    => None
+  end.
+
+Fixpoint merge_cfgps n :
+  forall (vd:svec desc n), shvec sdenote_desc_conc_pat vd ->
+      shvec sdenote_desc_conc_pat vd -> shvec sdenote_desc_conc_pat vd :=
+  match n as _n return
+    forall (vd:svec desc _n), shvec sdenote_desc_conc_pat vd ->
+      shvec sdenote_desc_conc_pat vd -> shvec sdenote_desc_conc_pat vd
+  with
+  | O => fun _ _ _ => tt
+  | S n' => fun vd =>
+    match vd as _vd return
+      shvec (n:=S n') sdenote_desc_conc_pat _vd ->
+      shvec (n:=S n') sdenote_desc_conc_pat _vd ->
+      shvec (n:=S n') sdenote_desc_conc_pat _vd
+    with
+    | (vd0, vd') => fun cfgp1 cfgp2 =>
+      (merge_desc_pats vd0 (fst cfgp1) (fst cfgp2), merge_cfgps n' vd' (snd cfgp1) (snd cfgp2))
+    end
+  end.
+
+Definition merge_all_cfgps ct cfgps cfgp0 :=
+  fold_right (merge_cfgps _ (projT2 (compd_conf (COMPS ct))))
+  cfgp0 cfgps.
+*)
+(*Definition get_ccomp_vals ct cfgps cfgp0 :=
+  {| conc_pat_type:=ct
+   ; conc_pat_conf:=fold_right
+       (merge_cfgps _ (projT2 (compd_conf (COMPS ct))))
+       cfgp0 cfgps |}.*)
+
+Lemma compcd_inj : forall ct ct',
+  Comp COMPT ct = Comp COMPT ct' ->
+  ct = ct'.
+Proof.
+  intros. injection H. auto.
+Qed.
+
+Definition peval_hdlr_term {cd envd} ct mt (t : hdlr_term ct mt envd cd)
+  (v:shvec sdenote_desc_conc_pat (projT2 (compd_conf (COMPS ct))))
+  : option (sdenote_cdesc COMPT COMPS cd).
+  destruct t.
+    exact None.
+    exact None.
+refine (
+  match t in Reflex.hdlr_term _ _ _ _ _ _ _ _c return
+      _c = Comp COMPT ct' -> _
+  with
+  | CComp => fun EQ =>
+    match compcd_inj _ _ EQ in _ = _ct return
+      forall (i:fin (projT1 (comp_conf_desc COMPT COMPS _ct))),
+      option
+      (sdenote_cdesc COMPT COMPS
+       (Desc COMPT (svec_ith (projT2 (comp_conf_desc COMPT COMPS _ct)) i)))
+    with
+    | Logic.eq_refl => fun i =>
+      shvec_ith _ _ v i
+    end i
+  | _ => fun _ => None
+  end (Logic.eq_refl _)).
+      exact None.
+    exact None.
+Defined.
+
+Lemma peval_hdlr_term_sound : forall cd envd ct mt
+  (t:hdlr_term ct mt envd cd) cfgp v cfg f pl,
+  peval_hdlr_term ct mt t cfgp = Some v ->
+  (forall i v,
+    shvec_ith sdenote_desc_conc_pat (projT2 (compd_conf (COMPS ct))) cfgp i =
+    Some v ->
+    shvec_ith sdenote_desc (projT2 (compd_conf (COMPS ct))) cfg i = v) ->
+  (forall st env,
+    eval_hdlr_term PAYD COMPT COMPS KSTD
+    (Build_comp COMPT COMPS ct f cfg)
+    (Build_msg PAYD mt pl) st t env = v).
+Proof.
+  intros cd envd ct mt t cfgp v cfg f pl Hpeval Hcfgp st env. Require Import Program.
+  generalize dependent v. dependent inversion t; try discriminate.
+  dependent destruction h; try discriminate. admit.
+  generalize dependent h0. (* rewrite <- x.
+  rewrite <- x0. generalize (Comp COMPT ct').
+
+revert x0. generalize (svec_ith (projT2 KSTD) i0).
+  intros c Heqc. dependent rewrite <- Heqc in h0.
+  dependent rewrite <- x0 in h0.
+  generalize dependent i.
+  simpl.
+
+dependent inversion h with (fun (hndx : cdesc COMPT)
+(hterm : Reflex.hdlr_term PAYD COMPT COMPS KSTD ct mt envd hndx) =>
+
+match hndx as _hndx return
+  sdenote_cdesc COMPT COMPS _hndx ->
+  Prop
+with
+| Comp ct1 => fun x =>
+
+forall (i : fin (projT1 (comp_conf_desc COMPT COMPS ct1)))
+     (v : sdenote_desc (svec_ith (projT2 (comp_conf_desc COMPT COMPS ct1)) i)),
+   match
+     h in (Reflex.hdlr_term _ _ _ _ _ _ _ _c)
+     return
+       (_c = Comp COMPT ct' ->
+        option
+          (sdenote_desc
+             (svec_ith (projT2 (comp_conf_desc COMPT COMPS ct1)) i)))
+   with
+   | Base d _ => fun _ : d = Comp COMPT ct' => None
+   | CComp =>
+       fun EQ : Comp COMPT ct = Comp COMPT ct' =>
+       match
+         compcd_inj ct ct' EQ in (_ = _ct)
+         return
+           (forall i0 : fin (projT1 (comp_conf_desc COMPT COMPS _ct)),
+            option
+              (sdenote_desc
+                 (svec_ith (projT2 (comp_conf_desc COMPT COMPS _ct)) i0)))
+       with
+       | eq_refl =>
+           fun i0 : fin (projT1 (comp_conf_desc COMPT COMPS ct)) =>
+           shvec_ith sdenote_desc_conc_pat (projT2 (compd_conf (COMPS ct)))
+             cfgp i0
+       end i
+   | CConf ct'0 i0 _ =>
+       fun
+         _ : Desc COMPT
+               (svec_ith (projT2 (comp_conf_desc COMPT COMPS ct'0)) i0) =
+             Comp COMPT ct' => None
+   | MVar i0 =>
+       fun
+         _ : Desc COMPT (svec_ith (projT2 (lkup_tag PAYD mt)) i0) =
+             Comp COMPT ct' => None
+   | StVar i0 => fun _ : svec_ith (projT2 KSTD) i0 = Comp COMPT ct' => None
+   end (eq_refl (Comp COMPT ct')) = Some v ->
+   match
+     projT2
+       x in (_ = _ct)
+     return
+       (forall _i : fin (projT1 (comp_conf_desc COMPT COMPS _ct)),
+        sdenote_desc (svec_ith (projT2 (comp_conf_desc COMPT COMPS _ct)) _i))
+   with
+   | eq_refl =>
+       fun
+         i0 : fin
+                (projT1
+                   (comp_conf_desc COMPT COMPS
+                      (comp_type COMPT COMPS
+                         (projT1
+                            x)))) =>
+       shvec_ith sdenote_desc
+         (projT2
+            (comp_conf_desc COMPT COMPS
+               (comp_type COMPT COMPS
+                  (projT1
+                     x))))
+         (comp_conf COMPT COMPS
+            (projT1
+               x)) i0
+   end i = v
+
+| _ => fun _ => True
+end
+
+(eval_hdlr_term PAYD COMPT COMPS KSTD
+                  {| comp_type := ct; comp_fd := f; comp_conf := cfg |}
+                  {| tag := mt; pay := pl |} st h env)
+
+).
+
+
+
+
+
+
+
+
+
+
+
+
+
+
+
+
+
+
+
+
+
+
+
+
+
+
+
+
+
+
+
+
+
+
+
+
+
+
+
+
+
+
+
+
+
+
+
+
+
+
+
+
+
+
+
+
+
+
+
+
+
+
+
+
+
+
+
+
+
+
+
+
+
+
+
+
+
+forall i : fin (projT1 (comp_conf_desc COMPT COMPS ct1)),
+   Desc COMPT (svec_ith (projT2 (comp_conf_desc COMPT COMPS ct1)) i) = cd ->
+   forall
+     v : sdenote_cdesc COMPT COMPS
+           (Desc COMPT (svec_ith (projT2 (comp_conf_desc COMPT COMPS ct1)) i)),
+   y = Some v ->
+match
+     projT2 x in (_ = _ct)
+     return
+       (forall _i : fin (projT1 (comp_conf_desc COMPT COMPS _ct)),
+        sdenote_desc (svec_ith (projT2 (comp_conf_desc COMPT COMPS _ct)) _i))
+   with
+   | eq_refl =>
+       fun
+         i0 : fin
+                (projT1
+                   (comp_conf_desc COMPT COMPS
+                      (comp_type COMPT COMPS
+                         (projT1 x)))) =>
+       shvec_ith sdenote_desc
+         (projT2
+            (comp_conf_desc COMPT COMPS
+               (comp_type COMPT COMPS
+                  (projT1 x))))
+         (comp_conf COMPT COMPS
+            (projT1 x)) i0
+   end i = v
+
+| _ => fun _ => True
+end
+
+(eval_hdlr_term PAYD COMPT COMPS KSTD
+                  {| comp_type := ct; comp_fd := f; comp_conf := cfg |}
+                  {| tag := mt; pay := pl |} st hterm env)
+
+). simpl. discriminate. simpl. admit. simpl. generalize (shvec_ith (sdenote_cdesc COMPT COMPS) (projT2 KSTD) st i). generalize (svec_ith (projT2 KSTD) i).
+
+  unfold eval_hdlr_term. simpl.
+  simpl. Require Import Program. simpl. dependent destruction h; try discriminate. admit. dependent inversion h. unfold eval_hdlr_term; simpl
+  intros v. 
+  rewrite UIP_refl with (p:=compcd_inj ct' ct' eq_refl). intro Hpeval. simpl in *. auto.
+(*apply JMeq_eq_dep in x; auto. apply eq_dep_eq_sigT in x. SearchAbout existT.
+   inversion x.*)*)
+  admit.
+Qed.
+
+Definition peval_expr {cd envd} ct mt
+  (e:expr COMPT (hdlr_term ct mt) envd cd)
+  (v:shvec sdenote_desc_conc_pat (projT2 (compd_conf (COMPS ct))))
+  : option (sdenote_cdesc COMPT COMPS cd).
+induction e.
+  exact (peval_hdlr_term ct mt t v).
+  
+  destruct IHe.
+    exact (Some (eval_unop COMPT COMPS _ _ u s)).
+    exact None.
+
+  destruct IHe1.
+    destruct IHe2.
+      exact (Some (eval_binop COMPT COMPS _ _ _ b s s0)).
+      exact None.
+
+    exact None.
+Defined.
+
+Lemma peval_expr_sound : forall cd envd ct mt
+  (e:expr COMPT (hdlr_term ct mt) envd cd) cfgp v cfg f pl,
+  peval_expr ct mt e cfgp = Some v ->
+  (forall i v,
+    shvec_ith sdenote_desc_conc_pat (projT2 (compd_conf (COMPS ct))) cfgp i =
+    Some v ->
+    shvec_ith sdenote_desc (projT2 (compd_conf (COMPS ct))) cfg i = v) ->
+  (forall st env,
+    eval_hdlr_expr PAYD COMPT COMPS KSTD
+    (Build_comp COMPT COMPS ct f cfg)
+    (Build_msg PAYD mt pl) st env e = v).
+Proof.
+  intros cd envd ct mt e cfgp v cfg f pl Hpeval Hcfgp st env.
+
+  induction e; simpl in *.
+    eapply peval_hdlr_term_sound with (v:=v); eauto.
+    
+    destruct (peval_expr ct mt e cfgp); try discriminate.
+    inversion Hpeval. rewrite IHe with (v:=s); auto.
+
+    destruct (peval_expr ct mt e1 cfgp); try discriminate;
+    destruct (peval_expr ct mt e2 cfgp); try discriminate.
+    inversion Hpeval. rewrite IHe1 with (v:=s); auto;
+    rewrite IHe2 with (v:=s0); auto.
+Qed.
+
+Definition peval_oexpr {cd envd} ct mt
+  (oe:option (expr COMPT (hdlr_term ct mt) envd cd))
+  (v:shvec sdenote_desc_conc_pat (projT2 (compd_conf (COMPS ct))))
+  : option (sdenote_cdesc COMPT COMPS cd).
+destruct oe.
+  exact (peval_expr ct mt e v).
+  exact None.
+Defined.
+
+Lemma peval_oexpr_sound : forall cd envd ct mt
+  (oe:option (expr COMPT (hdlr_term ct mt) envd cd)) cfgp v cfg f pl,
+  peval_oexpr ct mt oe cfgp = Some v ->
+  (forall i v,
+    shvec_ith sdenote_desc_conc_pat (projT2 (compd_conf (COMPS ct))) cfgp i =
+    Some v ->
+    shvec_ith sdenote_desc (projT2 (compd_conf (COMPS ct))) cfg i = v) ->
+  (forall st env,
+    eval_oexpr COMPT COMPS (hdlr_term ct mt)
+    (fun d envd env t =>
+      eval_hdlr_term PAYD COMPT COMPS KSTD
+      (Build_comp COMPT COMPS ct f cfg)
+      (Build_msg PAYD mt pl) st t env) env oe = Some v).
+Proof.
+  intros cd envd ct mt oe cfgp v cfg f pl Hpeval Hcfgp st env.
+  destruct oe; try discriminate.
+    simpl in *. f_equal.
+    pose proof (peval_expr_sound cd envd ct mt e cfgp v cfg f pl Hpeval Hcfgp st env).
+    unfold eval_hdlr_expr in *. auto.
+Qed.
+
+Fixpoint peval_payload_oexpr ct mt envd n : forall (vd:svec desc n),
+  payload_oexpr' COMPT (hdlr_term ct mt) envd n vd ->
+  shvec sdenote_desc_conc_pat (projT2 (compd_conf (COMPS ct))) ->
+  shvec sdenote_desc_conc_pat vd.
+intros vd cfgpe cfgp.
+induction n.
+  exact tt.
+
+  simpl in *. destruct vd as [vd0 vd']. destruct cfgpe as [oe cfgpe'].
+  exact (peval_oexpr ct mt oe cfgp, peval_payload_oexpr ct mt envd n vd' cfgpe' cfgp).
+Defined.
+
+Lemma peval_payload_oexpr_sound : forall envd ct mt vd
+  (cfgpe:payload_oexpr' COMPT (hdlr_term ct mt) envd (projT1 vd) (projT2 vd))
+  cfgp cfg f pl,
+  (forall i v,
+    shvec_ith sdenote_desc_conc_pat (projT2 (compd_conf (COMPS ct))) cfgp i =
+    Some v ->
+    shvec_ith sdenote_desc (projT2 (compd_conf (COMPS ct))) cfg i = v) ->
+  (forall st env,
+    cfgp_incl _
+     (eval_hdlr_payload_oexpr PAYD COMPT COMPS KSTD
+       (Build_comp COMPT COMPS ct f cfg)
+       (Build_msg PAYD mt pl) st envd env vd cfgpe)
+     (peval_payload_oexpr ct mt envd (projT1 vd) (projT2 vd) cfgpe cfgp)).
+Proof.
+  intros envd ct mt vd cfgpe cfgp cfg f pl Hcfgp st env cfg'.
+  apply Bool.leb_implb. unfold Bool.leb.
+  match goal with
+  |- if ?e then _ else _ =>
+    destruct e as [? | ?]_eqn; auto
+  end. destruct vd as [n vd].
+  induction n.
+    auto.
+
+    destruct vd. destruct cfgpe. destruct cfg'. simpl in *.
+    apply andb_prop in Heqb. destruct Heqb.
+    destruct (peval_oexpr ct mt o cfgp) as [? | ?]_eqn.
+      rewrite peval_oexpr_sound with (v:=s2) (cfgp:=cfgp) in H; auto.
+      rewrite H. simpl. apply IHn; auto.
+
+      simpl. apply IHn; auto.
+Qed.
+
+Definition is_high_comp_pat ct mt envd cp clblr cfgp : bool :=
+  let conf := peval_payload_oexpr ct _ _ _ _
+    (comp_pat_conf COMPT COMPS (hdlr_term ct mt) envd cp) 
+    cfgp in
+  let cpt := comp_pat_type _ _ _ _ cp in
+  match clblr cpt with
+  | Some cpcfgp =>
+    projT1 (bool_of_sumbool (cp_incl_dec (Build_conc_pat COMPT COMPS cpt conf)
+      (Build_conc_pat COMPT COMPS cpt cpcfgp)))
+  | None => false
+  end.
+
+(*  match get_candidate_pats clblr ct with
+  | cfg0::cfgs' =>
+    let merged := merge_all_cfgps ct cfgs' cfg0 in
+    let conf := get_conc_pat_conf ct _ _ _ _ (comp_pat_conf COMPT COMPS (hdlr_term ct mt) envd cp) merged in
+    existsb (fun cp' =>
+      (proj1_sig (bool_of_sumbool
+      (cp_incl_dec
+        (Build_conc_pat COMPT COMPS
+          (comp_pat_type _ _ _ _ cp) conf) cp')))) clblr
+  | nil => false
+  end.*)
+
+Lemma high_comp_cfgp_sound' : forall n vd v (i:fin n) cfg s,
+  shvec_match vd sdenote_desc sdenote_desc_conc_pat
+    elt_match cfg v = true ->
+  shvec_ith sdenote_desc_conc_pat vd v i = Some s ->
+  shvec_ith sdenote_desc vd cfg i = s.
+Proof.
+  intros n vd v i cfg s Hmatch Hith.
+  induction n.
+    contradiction.
+
+    destruct vd as [vd0 vd']. destruct cfg as [cfg0 cfg'].
+    destruct v as [v0 v']. simpl in *.
+    apply andb_prop in Hmatch. destruct Hmatch as [Hmatch_elt ?].
+    destruct i.
+      apply IHn with (v:=v'); auto.
+
+      rewrite Hith in Hmatch_elt. simpl in Hmatch_elt.
+      destruct vd0;
+        match goal with
+        | [ _ : context [ if ?e then _ else _ ] |- _ ]=>
+          destruct e; try discriminate; auto
+        end.
+Qed.
+
+Lemma high_comp_cfgp_sound : forall ct f cfg clblr,
+  lblr_match_comp COMPT COMPTDEC COMPS clblr
+  {| comp_type := ct; comp_fd := f; comp_conf := cfg |} = true ->
+  match clblr ct with
+  | Some cfgp =>
+    (forall (i : fin (projT1 (comp_conf_desc COMPT COMPS ct)))
+      (v : s[[svec_ith (projT2 (comp_conf_desc COMPT COMPS ct)) i]]),
+      shvec_ith sdenote_desc_conc_pat (projT2 (comp_conf_desc COMPT COMPS ct))
+      cfgp i = Some v ->
+      shvec_ith sdenote_desc (projT2 (comp_conf_desc COMPT COMPS ct)) cfg i = v)
+  | None => True
+  end.
+Proof.
+  intros ct f cfg clblr Hlblr.
+  unfold lblr_match_comp, match_comp,
+    Reflex.match_comp, match_comp_pf in Hlblr. simpl in *.
+  destruct (clblr ct); auto.
+  destruct (COMPTDEC ct ct); try discriminate.
+  rewrite UIP_refl with (p:=e) in Hlblr. intros.
+  apply high_comp_cfgp_sound' with (v:=s); auto.
+  match goal with
+  |- ?e = true =>
+    destruct e; try discriminate; auto
+  end.
+Qed.
+
+Lemma is_high_comp_pat_sound : forall c m envd cp cfgp clblr,
+  lblr_match_comp COMPT COMPTDEC COMPS clblr c = true ->
+  clblr (comp_type _ _ c) = Some cfgp ->
+  is_high_comp_pat (comp_type _ _ c) (tag _ m) envd cp clblr cfgp = true ->
+  forall st env,
+    high_comp_pat COMPT COMPTDEC COMPS
+      (eval_hdlr_comp_pat PAYD COMPT COMPS KSTD c m st envd env cp)
+      (lblr_match_comp COMPT COMPTDEC COMPS clblr).
+Proof.
+  intros c m envd cp cfgp clblr Hmatch Hcfgp Hhigh st env.
+  unfold is_high_comp_pat in Hhigh.
+  destruct cp as [cpt cpfg]. destruct c as [ct f cfg].
+  destruct m as [mt pl]. simpl in *.
+  unfold high_comp_pat. intros c' Hmatch'.
+  destruct (clblr cpt) as [ ? | ? ]_eqn; try discriminate.
+  match goal with
+  | [ _ : context [ cp_incl_dec ?cp1 ?cp2 ] |- _ ]
+    => destruct (cp_incl_dec cp1 cp2); try discriminate
+  end. unfold cp_incl in *. clear Hhigh. specialize (c c').
+  unfold match_comp, Reflex.match_comp, match_comp_pf in *.
+  simpl in *. unfold hdlr_term, CT, CTAG in *.
+  destruct c' as [ct' ? ?]. simpl in *.
+  destruct (COMPTDEC ct' cpt); try discriminate.
+  subst ct'.
+  pose proof (high_comp_cfgp_sound ct f cfg clblr Hmatch).
+  rewrite Hcfgp in *.
+  pose proof (peval_payload_oexpr_sound envd ct mt _
+    cpfg cfgp cfg f pl H st env).
+  unfold lblr_match_comp, Reflex.match_comp, match_comp_pf. simpl in *.
+  destruct (COMPTDEC cpt cpt); try intuition.
+  rewrite UIP_refl with (p:=e). rewrite Heqo.
+  unfold cfgp_incl in *. simpl in *. specialize (H0 comp_conf).
+  destruct
+    (shvec_match
+           (projT2 (comp_conf_desc COMPT COMPS cpt))
+           sdenote_desc sdenote_desc_conc_pat elt_match
+           comp_conf
+           (eval_hdlr_payload_oexpr PAYD COMPT COMPS KSTD
+              {| comp_type := ct; comp_fd := f; comp_conf := cfg |}
+              {| tag := mt; pay := pl |} st envd env
+              (comp_conf_desc COMPT COMPS cpt) cpfg));
+    try discriminate. simpl in *. rewrite H0 in *. auto.
+Qed.
+
+Definition lift_llblr n llblr b : fin (S n) -> bool :=
+  fun i => 
+    match fin_eq_dec i (max_fin n) with
+    | left _ => b
+    | right H => llblr (proj_fin_ok i H)
+    end.
+
+Fixpoint get_llblr ct mt envd cmd cfgp clblr vlblr llblr :=
+  match cmd in Reflex.cmd _ _ _ _ _ _envd return
+    (fin (projT1 _envd) -> bool) -> _
+  with
+  | Reflex.Seq _ cmd1 cmd2 => fun llblr =>
+    let llblr1 := get_llblr ct mt _ cmd1 cfgp clblr vlblr llblr in
+    get_llblr ct mt _ cmd2 cfgp clblr vlblr llblr1
+  | Reflex.Ite envd e cmd1 cmd2 => fun llblr =>
+    if hdlr_expr_ok_high ct mt envd _ e vlblr llblr
+    then fun i => andb (get_llblr ct mt _ cmd1 cfgp clblr vlblr llblr i)
+      (get_llblr ct mt _ cmd2 cfgp clblr vlblr llblr i)
+    else fun i => andb (get_writes _ _ cmd1 i) (get_writes _ _ cmd2 i)
+  | Reflex.CompLkup envd cp i' EQ cmd1 cmd2 => fun llblr =>
+    if andb (is_high_comp_pat ct mt _ cp clblr cfgp)
+         (pl_oexpr_ok_high ct mt _ _ _
+           (comp_pat_conf _ _ _ _ cp) vlblr llblr)
+    then fun i => andb
+      (get_llblr ct mt _ cmd1 cfgp clblr vlblr
+        (fun i => if fin_eq_dec i i' then true else llblr i) i)
+      (get_llblr ct mt _ cmd2 cfgp clblr vlblr llblr i)
+    else fun i => andb (get_writes _ _ cmd1 i) (get_writes _ _ cmd2 i)
+  | Reflex.Spawn _ t e i _ => fun llblr =>
+    if pl_expr_ok_high ct mt _ _ _ e vlblr llblr
+    then fun i' =>
+      if fin_eq_dec i i'
+      then true
+      else llblr i'
+    else fun i' =>
+      if fin_eq_dec i i'
+      then false
+      else llblr i'
+  | _       => fun llblr => llblr
+  end llblr.
 
 Ltac uninhabit :=
   match goal with
@@ -44,6 +1013,952 @@ Ltac remove_redundant_ktr :=
       H' : Reflex.ktr _ _ _ _ ?s = inhabits ?tr' |- _ ]
     => rewrite H' in H; apply pack_injective in H; subst tr
   end.
+
+Lemma vlblr_shift : forall n (vlblr:fin (S n) -> bool) (f:fin n),
+  vlblr (Some f) = vlblr (shift_fin f).
+Proof.
+  intros n vlblr f.
+  induction n.
+    simpl in *. contradiction.
+
+    simpl. destruct f; auto.
+Qed.
+
+Definition states_ok (s1 s2:kstate) clblr vlblr :=
+  let clblr := lblr_match_comp COMPT COMPTDEC COMPS clblr in
+  high_out_eq _ _ _ _ s1 s2 clblr /\
+    vars_eq _ _ _ _ s1 s2 vlblr.
+
+Definition cmd_ok_low c m envd cmd clblr vlblr :=
+  forall env s i,
+    ReachInter s ->
+    lblr_match_comp COMPT COMPTDEC COMPS clblr c = false ->
+    states_ok s (hdlr_kst _ _ _ _ _ (ve_st c m envd cmd i {|hdlr_env:=env;hdlr_kst:=s|})) clblr vlblr.
+
+Definition cmd_ok_high c m envd cmd clblr vlblr llblr
+  (Hmatch:lblr_match_comp COMPT COMPTDEC COMPS clblr c = true) :=
+  forall env1 env2 s1 s2 i,
+    ReachInter s1 -> ReachInter s2 ->
+    states_ok s1 s2 clblr vlblr ->
+    locals_eq envd env1 env2 llblr ->
+    states_ok
+      (hdlr_kst _ _ _ _ _ (ve_st c m envd cmd i {|hdlr_env:=env1;hdlr_kst:=s1|}))
+      (hdlr_kst _ _ _ _ _ (ve_st c m envd cmd i {|hdlr_env:=env2;hdlr_kst:=s2|}))
+      clblr vlblr.
+
+Lemma shvec_erase_ith : forall n vlblr
+  (vd:svec (cdesc COMPT) n) v1 v2,
+  shvec_erase (sdenote_cdesc COMPT COMPS) vlblr vd v1 =
+  shvec_erase (sdenote_cdesc COMPT COMPS) vlblr vd v2 <->
+  (forall i, vlblr i = true ->
+    shvec_ith (sdenote_cdesc COMPT COMPS) vd v1 i =
+    shvec_ith (sdenote_cdesc COMPT COMPS) vd v2 i).
+Proof.
+  intros n vlblr vd v1 v2.
+  induction n.
+    split; intros; auto.
+
+    split.
+      intros Heq i Hlblr.
+      destruct vd; destruct i; simpl in *.
+        destruct v1; destruct v2; simpl in *.
+      apply IHn with (vlblr:=fun f => vlblr (shift_fin f));
+        auto. 
+      match goal with
+      | [ _ : context [ if ?e then _ else _ ] |- _ ]
+        => destruct e
+      end; inversion Heq; auto.
+      rewrite <- vlblr_shift; auto.
+
+      rewrite Hlblr in *. inversion Heq. auto.
+
+      intro H. destruct vd. simpl.
+      match goal with
+      |- context [ if ?e then _ else _ ]
+        => destruct e as [? | ?]_eqn
+      end. f_equal. apply (H None Heqb).
+      apply IHn; auto.
+      intros i Hi.
+      rewrite <- vlblr_shift in Hi.
+      apply (H (Some i) Hi).
+
+      f_equal. apply IHn; auto.
+      intros i Hi.
+      rewrite <- vlblr_shift in Hi.
+      apply (H (Some i) Hi).
+Qed.
+
+Lemma hdlr_expr_ok_high_correct : forall c m (envd:vcdesc COMPT) cd
+  (e:expr _ (hdlr_term (CT _ COMPS c) (CTAG PAYD m)) envd cd)
+  clblr vlblr llblr s1 s2 (env1 env2:sdenote_vcdesc _ _ envd),
+  hdlr_expr_ok_high _ _ _ _ e vlblr llblr = true ->
+  states_ok s1 s2 clblr vlblr ->
+  locals_eq envd env1 env2 llblr ->
+  eval_hdlr_expr _ _ _ _ _ _ (kst _ _ _ _ s1) env1 e =
+  eval_hdlr_expr _ _ _ _ _ _ (kst _ _ _ _ s2) env2 e.
+Proof.
+  intros c m envd cd e clblr vlblr llblr s1 s2 env1 env2 Hexpr Hstates Hlocals.
+  induction e; simpl in *.
+    induction t; simpl in *; auto; try discriminate.
+      destruct b; simpl in *; auto; try discriminate.
+      unfold locals_eq in Hlocals. destruct envd as [? envd]. simpl.
+      eapply shvec_erase_ith with (vd:=envd) (i:=i); eauto.
+
+      rewrite IHt; auto.
+
+      destruct Hstates as [Hout Hvars]. unfold vars_eq in Hvars.
+      destruct s1; destruct s2; destruct KSTD; simpl.
+      eapply shvec_erase_ith with (vd:=v) (v1:=kst)
+        (v2:=kst0) (i:=i); eauto.
+
+    rewrite IHe; auto.
+
+    apply andb_prop in Hexpr. destruct Hexpr.
+    rewrite IHe1; auto. rewrite IHe2; auto.
+Qed.
+
+Lemma hdlr_oexpr_ok_high_correct : forall c m (envd:vcdesc COMPT) cd
+  (oe:option (expr _ (hdlr_term (CT _ COMPS c) (CTAG PAYD m)) envd cd))
+  clblr vlblr llblr s1 s2 (env1 env2:sdenote_vcdesc _ _ envd),
+  hdlr_oexpr_ok_high _ _ _ _ oe vlblr llblr = true ->
+  states_ok s1 s2 clblr vlblr ->
+  locals_eq envd env1 env2 llblr ->
+  eval_oexpr COMPT COMPS (hdlr_term (CT _ COMPS c) (CTAG PAYD m))
+    (fun d envd env t =>
+      eval_hdlr_term PAYD COMPT COMPS KSTD
+      c m (kst _ _ _ _ s1) t env) env1 oe =
+  eval_oexpr COMPT COMPS (hdlr_term (CT _ COMPS c) (CTAG PAYD m))
+    (fun d envd env t =>
+      eval_hdlr_term PAYD COMPT COMPS KSTD
+      c m (kst _ _ _ _ s2) t env) env2 oe.
+Proof.
+  intros c m envd cd oe clblr vlblr llblr s1 s2 env1 env2 Hexpr Hstates Hlocals.
+  destruct oe.
+    simpl in *. f_equal.
+    apply (hdlr_expr_ok_high_correct c m envd cd e
+      clblr vlblr llblr s1 s2 env1 env2); auto.
+
+    auto.
+Qed.
+
+Lemma expr_list_ok_high_correct : forall c m (envd:vcdesc COMPT) cd
+  (es:list (expr _ (hdlr_term (CT _ COMPS c) (CTAG PAYD m)) envd cd))
+  clblr vlblr llblr s1 s2 (env1 env2:sdenote_vcdesc _ _ envd),
+  expr_list_ok_high _ _ _ _ es vlblr llblr = true ->
+  states_ok s1 s2 clblr vlblr ->
+  locals_eq envd env1 env2 llblr ->
+  map (eval_hdlr_expr _ _ _ _ _ _ (kst _ _ _ _ s1) env1) es =
+  map (eval_hdlr_expr _ _ _ _ _ _ (kst _ _ _ _ s2) env2) es.
+Proof.
+  intros c m envd cd es clblr vlblr llblr
+    s1 s2 env1 env2 Hexpr Hstates Hlocals.
+  induction es.
+    auto.
+
+    simpl in *.
+    destruct (hdlr_expr_ok_high (CT COMPT COMPS c) (CTAG PAYD m) envd cd a vlblr
+             llblr) as [? | ?]_eqn; try discriminate.
+    erewrite hdlr_expr_ok_high_correct; eauto.
+    rewrite IHes; auto.
+Qed.
+
+Lemma pl_hdlr_expr_ok_high_correct : forall c m (envd:vcdesc COMPT) vd
+  (e:payload_expr _ (hdlr_term (CT _ COMPS c) (CTAG PAYD m)) envd vd)
+  clblr vlblr llblr s1 s2 (env1 env2:sdenote_vcdesc _ _ envd),
+  pl_expr_ok_high _ _ _ _ (projT2 vd) e vlblr llblr = true ->
+  states_ok s1 s2 clblr vlblr ->
+  locals_eq envd env1 env2 llblr ->
+  eval_hdlr_payload_expr _ _ _ _ _ _ (kst _ _ _ _ s1) _ env1 _ e =
+  eval_hdlr_payload_expr _ _ _ _ _ _ (kst _ _ _ _ s2) _ env2 _ e.
+Proof.
+  intros c m envd vd e clblr vlblr llblr s1 s2 env1 env2 Hexpr Hstates Hlocals.
+  destruct vd as [n vd].
+  induction n.
+    auto.
+
+    destruct vd. destruct e.
+    unfold eval_hdlr_payload_expr, eval_payload_expr, eval_payload_expr' in *.
+    simpl in *. apply andb_prop in Hexpr. destruct Hexpr as [Hfst ?].
+    eapply hdlr_expr_ok_high_correct in Hfst; eauto.
+    unfold eval_hdlr_expr in Hfst. simpl in *. rewrite Hfst.
+    f_equal. apply IHn; auto.
+Qed.
+
+Lemma pl_hdlr_oexpr_ok_high_correct : forall c m (envd:vcdesc COMPT) vd
+  (oe:payload_oexpr _ (hdlr_term (CT _ COMPS c) (CTAG PAYD m)) envd vd)
+  clblr vlblr llblr s1 s2 (env1 env2:sdenote_vcdesc _ _ envd),
+  pl_oexpr_ok_high _ _ _ _ (projT2 vd) oe vlblr llblr = true ->
+  states_ok s1 s2 clblr vlblr ->
+  locals_eq envd env1 env2 llblr ->
+  eval_hdlr_payload_oexpr _ _ _ _ _ _ (kst _ _ _ _ s1) _ env1 _ oe =
+  eval_hdlr_payload_oexpr _ _ _ _ _ _ (kst _ _ _ _ s2) _ env2 _ oe.
+Proof.
+  intros c m envd vd e clblr vlblr llblr s1 s2 env1 env2 Hexpr Hstates Hlocals.
+  destruct vd as [n vd].
+  induction n.
+    auto.
+
+    destruct vd. destruct e.
+    unfold eval_hdlr_payload_oexpr, eval_payload_oexpr, eval_payload_oexpr' in *.
+    simpl in *. apply andb_prop in Hexpr. destruct Hexpr as [Hfst ?].
+    eapply hdlr_oexpr_ok_high_correct in Hfst; eauto.
+    simpl in *. f_equal. auto.
+    apply IHn; auto.
+Qed.
+
+Definition get_ccomp_cfgp c clblr
+  (Hmatch:lblr_match_comp COMPT COMPTDEC COMPS clblr c = true) :
+  shvec sdenote_desc_conc_pat (projT2 (compd_conf (COMPS (comp_type _ _ c)))).
+unfold lblr_match_comp in Hmatch.
+destruct (clblr (comp_type _ _ c)).
+  exact s.
+  discriminate.
+Defined.
+
+Lemma get_ccomp_cfgp_correct : forall c clblr
+  (Hmatch:lblr_match_comp COMPT COMPTDEC COMPS clblr c = true),
+  clblr (comp_type COMPT COMPS c) = Some (get_ccomp_cfgp c clblr Hmatch).
+Proof.
+  intros c clblr Hmatch.
+  unfold lblr_match_comp in Hmatch.
+  destruct c as [ct ? ?]. simpl in *. unfold get_ccomp_cfgp.
+  simpl. destruct (clblr ct); auto; discriminate.
+Qed.
+
+Fixpoint all_cmd_ok_high c m envd
+  cmd clblr vlblr llblr
+  (Hmatch:lblr_match_comp COMPT COMPTDEC COMPS clblr c = true) : Prop :=
+  let ccfgp := get_ccomp_cfgp c clblr Hmatch in
+  match cmd in Reflex.cmd _ _ _ _ _ _envd return
+    (fin (projT1 _envd) -> bool) -> _
+  with
+  | Reflex.Seq _ cmd1 cmd2 => fun llblr =>
+    all_cmd_ok_high c m _ cmd1 clblr vlblr llblr Hmatch /\
+    all_cmd_ok_high c m _ cmd2 clblr vlblr
+      (get_llblr _ _ _ cmd1 ccfgp clblr vlblr llblr) Hmatch
+  | Reflex.Ite _ e cmd1 cmd2 => fun llblr =>
+    if hdlr_expr_ok_high _ _ _ _ e vlblr llblr
+    then all_cmd_ok_high c m _ cmd1 clblr vlblr llblr Hmatch /\
+      all_cmd_ok_high c m _ cmd2 clblr vlblr llblr Hmatch
+    else False
+  | Reflex.CompLkup _ cp i' EQ cmd1 cmd2 => fun llblr =>
+    if andb (is_high_comp_pat (comp_type _ _ c) (tag _ m) _ cp clblr ccfgp)
+         (pl_oexpr_ok_high (comp_type _ _ c) (tag _ m) _ _ _
+           (comp_pat_conf _ _ _ _ cp) vlblr llblr)
+    then all_cmd_ok_high c m _ cmd1 clblr vlblr
+      (fun i => if fin_eq_dec i i' then true else llblr i) Hmatch /\
+      all_cmd_ok_high c m _ cmd2 clblr vlblr llblr Hmatch
+    else False
+  | _ => fun _ => cmd_ok_high c m envd cmd clblr vlblr llblr Hmatch
+  end llblr.
+
+Definition cmd_ok_high' c m envd cmd clblr vlblr llblr
+  (Hmatch:lblr_match_comp COMPT COMPTDEC COMPS clblr c = true) :=
+  forall env1 env2 s1 s2 i,
+    ReachInter s1 -> ReachInter s2 ->
+    states_ok s1 s2 clblr vlblr ->
+    locals_eq envd env1 env2 llblr ->
+    states_ok
+      (hdlr_kst _ _ _ _ _ (ve_st c m envd cmd i {|hdlr_env:=env1;hdlr_kst:=s1|}))
+      (hdlr_kst _ _ _ _ _ (ve_st c m envd cmd i {|hdlr_env:=env2;hdlr_kst:=s2|}))
+      clblr vlblr /\
+    locals_eq envd
+      (hdlr_env _ _ _ _ _ (ve_st c m envd cmd i {|hdlr_env:=env1;hdlr_kst:=s1|}))
+      (hdlr_env _ _ _ _ _ (ve_st c m envd cmd i {|hdlr_env:=env2;hdlr_kst:=s2|}))
+      (get_llblr _ _ _ cmd (get_ccomp_cfgp c clblr Hmatch) clblr vlblr llblr).
+
+Lemma cmd_ok_high'_ok : forall c m envd cmd clblr vlblr llblr Hmatch,
+  cmd_ok_high' c m envd cmd clblr vlblr llblr Hmatch ->
+  cmd_ok_high c m envd cmd clblr vlblr llblr Hmatch.
+Proof.
+  unfold cmd_ok_high, cmd_ok_high'. intros.
+  apply H; auto.
+Qed.
+
+Lemma shvec_erase_wklblr : forall n lblr lblr'
+  (vd:svec (cdesc COMPT) n) v1 v2,
+  (forall i, implb (lblr' i) (lblr i) = true) ->
+  shvec_erase (sdenote_cdesc COMPT COMPS) lblr vd v1 =
+  shvec_erase (sdenote_cdesc COMPT COMPS) lblr vd v2 ->
+  shvec_erase (sdenote_cdesc COMPT COMPS) lblr' vd v1 =
+  shvec_erase (sdenote_cdesc COMPT COMPS) lblr' vd v2.
+Proof.
+  intros n lblr lblr' vd v1 v2 Himpl Herase.
+  rewrite shvec_erase_ith. rewrite shvec_erase_ith in Herase.
+  intros i Hlblr. apply Herase. specialize (Himpl i).
+  rewrite Hlblr in Himpl. unfold implb in Himpl. auto.
+Qed.
+
+Lemma all_cmd_ok_high_correct : forall c m envd cmd clblr vlblr llblr Hmatch,
+  all_cmd_ok_high c m envd cmd clblr vlblr llblr Hmatch ->
+  cmd_ok_high' c m envd cmd clblr vlblr llblr Hmatch.
+Proof.
+  intros c m envd cmd clblr vlblr llblr Hmatch Hall_ok. unfold cmd_ok_high'.
+  induction cmd; simpl in *; try abstract auto.
+    abstract (
+    intros; destruct Hall_ok as [Hall_ok1 Hall_ok2];
+    match goal with
+    |- context [ states_ok (hdlr_kst _ _ _ _ _
+      (ve_st _ _ _ _ _ ?s1)) (hdlr_kst _ _ _ _ _
+        (ve_st _ _ _ _ _ ?s2)) _ _ ]
+     => destruct s1 as [s1' env1']_eqn; destruct s2 as [s2' env2']_eqn
+    end; apply IHcmd2; auto;
+      try (
+      apply f_equal with (f:=hdlr_kst _ _ _ _ _)in Heqh;
+      apply f_equal with (f:=hdlr_kst _ _ _ _ _)in Heqh0;
+      simpl in *; subst s1'; subst s2'; destruct i; simpl;
+      specialize (IHcmd1 llblr Hall_ok1 env1 env2 s1 s2 s H H0);
+      apply IHcmd1; auto);
+      try (
+      apply f_equal with (f:=hdlr_env _ _ _ _ _)in Heqh;
+      apply f_equal with (f:=hdlr_env _ _ _ _ _)in Heqh0;
+      simpl in *; subst env1'; subst env2'; destruct i; simpl;
+      specialize (IHcmd1 llblr Hall_ok1 env1 env2 s1 s2 s H H0); apply IHcmd1; auto);
+      try (
+      apply f_equal with (f:=hdlr_kst _ _ _ _ _)in Heqh;
+        unfold ve_st in Heqh; simpl in Heqh; subst s1';
+          destruct i; simpl; destruct s1 as [? [k] ?];
+            apply ReachInter_run with (tr:=k); auto);
+      try (
+      apply f_equal with (f:=hdlr_kst _ _ _ _ _)in Heqh0;
+        unfold ve_st in Heqh0; simpl in Heqh0; subst s2';
+          destruct i; simpl; destruct s2 as [? [k] ?];
+            apply ReachInter_run with (tr:=k); auto)).
+
+    intros. destruct (hdlr_expr_ok_high (CT COMPT COMPS c) 
+    (CTAG PAYD m) envd (Desc COMPT num_d) e vlblr llblr) as [? | ?]_eqn.
+    destruct Hall_ok as [Hall_ok1 Hall_ok2].
+      erewrite hdlr_expr_ok_high_correct; eauto.
+      destruct (num_eq
+              (eval_hdlr_expr PAYD COMPT COMPS KSTD c m
+                 (kst PAYD COMPT COMPS KSTD s2) env2 e) FALSE).
+      unfold locals_eq in *.
+      split.
+        eapply IHcmd2; eauto.
+        apply shvec_erase_wklblr with
+          (lblr:=get_llblr (CT COMPT COMPS c) (CTAG PAYD m) envd cmd2
+            (get_ccomp_cfgp c clblr Hmatch) clblr vlblr
+                llblr). intros.
+        destruct (get_llblr (CT COMPT COMPS c) (CTAG PAYD m) envd cmd1
+          (get_ccomp_cfgp c clblr Hmatch) clblr vlblr llblr i0);
+        destruct (get_llblr (CT COMPT COMPS c) (CTAG PAYD m) envd cmd2 
+          (get_ccomp_cfgp c clblr Hmatch) clblr vlblr llblr i0);
+          auto.
+        apply IHcmd2; auto.
+
+      unfold locals_eq in *.
+      split.
+        eapply IHcmd1; eauto.
+        apply shvec_erase_wklblr with
+          (lblr:=get_llblr (CT COMPT COMPS c) (CTAG PAYD m) envd cmd1
+            (get_ccomp_cfgp c clblr Hmatch) clblr vlblr
+                llblr). intros.
+        destruct (get_llblr (CT COMPT COMPS c) (CTAG PAYD m) envd cmd2
+          (get_ccomp_cfgp c clblr Hmatch) clblr vlblr llblr i0);
+        destruct (get_llblr (CT COMPT COMPS c) (CTAG PAYD m) envd cmd1
+          (get_ccomp_cfgp c clblr Hmatch) clblr vlblr llblr i0);
+          auto.
+        apply IHcmd1; auto.
+
+      contradiction.
+
+    unfold cmd_ok_high in *. simpl in *. auto.
+
+    intros. split.
+      unfold cmd_ok_high in *. simpl in *. auto.
+
+      unfold locals_eq in *.
+      apply shvec_erase_ith.
+      destruct (pl_expr_ok_high (CT COMPT COMPS c) (CTAG PAYD m) envd
+        (projT1 (comp_conf_desc COMPT COMPS t))
+        (projT2 (comp_conf_desc COMPT COMPS t)) p vlblr llblr) as [? | ?]_eqn.
+        erewrite pl_hdlr_expr_ok_high_correct; eauto.
+        intros i' ?.
+        destruct (fin_eq_dec i i').
+          subst i'. repeat rewrite shvec_ith_replace_cast_ith. auto.
+          repeat rewrite shvec_ith_replace_cast_other; auto. rewrite shvec_erase_ith in H2. auto.
+
+          intros i' ?. destruct (fin_eq_dec i i'); try discriminate; try contradiction.
+          repeat rewrite shvec_ith_replace_cast_other; auto. rewrite shvec_erase_ith in H2.
+          auto.
+
+    intros. split.
+      unfold cmd_ok_high in *. simpl in *. auto.
+    
+      unfold locals_eq in *.
+      apply shvec_erase_ith.
+      intros i' ?.
+      destruct (fin_eq_dec i i').
+        subst i'. repeat rewrite shvec_ith_replace_cast_ith. auto.
+        repeat rewrite shvec_ith_replace_cast_other; auto.
+        rewrite shvec_erase_ith in H2. auto.
+
+    unfold cmd_ok_high in *. simpl in *. auto.
+
+    unfold CT, CTAG in *. simpl in *. intros.
+    destruct (is_high_comp_pat (comp_type COMPT COMPS c) 
+      (tag PAYD m) envd cp clblr (get_ccomp_cfgp c clblr Hmatch))
+      as [? | ?]_eqn; try contradiction.
+    unfold hdlr_term in *.
+    match goal with
+    | [ _ : context[pl_oexpr_ok_high ?a ?b ?c ?d ?e ?f ?g ?h] |- _ ]
+      => destruct (pl_oexpr_ok_high a b c d e f g h) as [? | ?]_eqn;
+        try contradiction
+    end.
+    destruct Hall_ok as [Hall_ok1 Hall_ok2]. intros.
+      unfold eval_hdlr_comp_pat. destruct cp as [cpt cpconf]_eqn. simpl.
+      rewrite (pl_hdlr_oexpr_ok_high_correct c m envd _
+        cpconf clblr vlblr llblr s1 s2 env1 env2); auto.
+      rewrite (hout_eq_find_eq PAYD COMPT COMPTDEC COMPS KSTD
+        ({|
+            conc_pat_type := cpt;
+            conc_pat_conf := eval_hdlr_payload_oexpr PAYD COMPT COMPS KSTD c
+                               m (kst PAYD COMPT COMPS KSTD s2) envd env2
+                               (comp_conf_desc COMPT COMPS cpt) cpconf |})
+        s1 s2 (lblr_match_comp COMPT COMPTDEC COMPS clblr)); auto.
+      match goal with
+      |- context [find_comp ?a ?b ?c ?d ?e] =>
+        destruct (find_comp a b c d e)
+      end.
+        unfold locals_eq in *.
+        split.
+          eapply IHcmd1; eauto.
+            destruct s1; auto.
+            destruct s2; eauto.
+            apply shvec_erase_ith. intros i' ?.
+            destruct (fin_eq_dec i' i).
+              subst i'. repeat rewrite shvec_ith_replace_cast_ith. auto.
+              repeat rewrite shvec_ith_replace_cast_other; auto.
+              rewrite shvec_erase_ith in H2. auto.
+
+          apply shvec_erase_wklblr with
+            (lblr:=get_llblr (comp_type COMPT COMPS c) (tag PAYD m) envd cmd1
+              (get_ccomp_cfgp c clblr Hmatch) clblr vlblr
+              (fun i1 : fin (projT1 envd) =>
+                if fin_eq_dec i1 i then true else llblr i1)). intros.
+          destruct ((get_llblr (comp_type COMPT COMPS c) (tag PAYD m) envd cmd1
+            (get_ccomp_cfgp c clblr Hmatch) clblr vlblr
+            (fun i2 : fin (projT1 envd) =>
+              if fin_eq_dec i2 i then true else llblr i2) i1)); auto.
+          destruct (get_llblr (comp_type COMPT COMPS c) (tag PAYD m) envd cmd2
+            (get_ccomp_cfgp c clblr Hmatch) clblr vlblr
+            llblr i1); auto.
+          eapply IHcmd1; eauto.
+          destruct s1; auto. destruct s2; auto.
+          apply shvec_erase_ith. intros i' ?.
+          destruct (fin_eq_dec i' i).
+            subst i'. repeat rewrite shvec_ith_replace_cast_ith. auto.
+            repeat rewrite shvec_ith_replace_cast_other; auto.
+            rewrite shvec_erase_ith in H2; auto.
+
+      split.
+        eapply IHcmd2; eauto.
+
+        unfold locals_eq in *.
+        apply shvec_erase_wklblr with
+          (lblr:=get_llblr (comp_type COMPT COMPS c) (tag PAYD m) envd cmd2
+            (get_ccomp_cfgp c clblr Hmatch) clblr vlblr
+            llblr). intros.
+        destruct (get_llblr (comp_type COMPT COMPS c) (tag PAYD m) envd cmd2
+          (get_ccomp_cfgp c clblr Hmatch) clblr vlblr
+          llblr i1);
+        destruct (get_llblr (comp_type COMPT COMPS c) (tag PAYD m) envd cmd1
+          (get_ccomp_cfgp c clblr Hmatch) clblr vlblr
+          (fun i2 : fin (projT1 envd) =>
+            if fin_eq_dec i2 i then true else llblr i2) i1); auto.
+        eapply IHcmd2; eauto.
+
+      apply H1.
+
+      pose proof (is_high_comp_pat_sound c m envd cp (get_ccomp_cfgp c clblr Hmatch) clblr) as Hgoal.
+      unfold eval_hdlr_comp_pat in *. subst cp. apply Hgoal; auto.
+      apply get_ccomp_cfgp_correct.
+Qed.
+
+Lemma complkup_low : forall c m envd clblr vlblr
+  cp i EQ cmd1 cmd2,
+  cmd_ok_low c m envd cmd1 clblr vlblr ->
+  cmd_ok_low c m envd cmd2 clblr vlblr ->
+  cmd_ok_low c m envd (CompLkup _ envd cp i EQ cmd1 cmd2) clblr vlblr.
+Proof.
+  intros c m envd clblr vlblr cp i EQ cmd1 cmd2 Hcmd1 Hcmd2.
+  unfold cmd_ok_low in *. intros. simpl.
+  destruct (find_comp COMPT COMPTDEC COMPS
+            (eval_hdlr_comp_pat PAYD COMPT COMPS KSTD c m
+               (kst PAYD COMPT COMPS KSTD s) envd env cp)
+            (kcs PAYD COMPT COMPS KSTD s)); auto.
+  destruct s; auto.
+Qed.
+
+Lemma complkup_high_all : forall c m envd clblr vlblr llblr
+  cp i EQ cmd1 cmd2 Hmatch,
+  is_high_comp_pat (comp_type _ _ c) (tag _ m) _ cp clblr
+    (get_ccomp_cfgp c clblr Hmatch) = true ->
+  pl_oexpr_ok_high (comp_type _ _ c) (tag _ m) _ _ _
+    (comp_pat_conf _ _ _ _ cp) vlblr llblr = true ->
+  all_cmd_ok_high c m envd cmd1 clblr vlblr
+    (fun i' : fin (projT1 envd) =>
+      if fin_eq_dec i' i then true else llblr i') Hmatch ->
+  all_cmd_ok_high c m envd cmd2 clblr vlblr llblr Hmatch ->
+  all_cmd_ok_high c m envd (CompLkup _ envd cp i EQ cmd1 cmd2) clblr vlblr llblr Hmatch.
+Proof.
+  intros c m envd clblr vlblr llblr cp i EQ
+    cmd1 cmd2 Hmatch Hhigh_pat Hhigh_conf Hcmd1 Hcmd2.
+  simpl. rewrite Hhigh_pat. unfold hdlr_term in *.
+  unfold CT. unfold CTAG. rewrite Hhigh_conf. simpl.
+  auto.
+Qed.
+
+Lemma stupd_low : forall clblr vlblr c m envd i e,
+  vlblr i = false ->
+  cmd_ok_low c m envd (StUpd _ _ i e) clblr vlblr.
+Proof.
+  intros clblr vlblr c m envd i e Hvar.
+  split.
+    unfold high_out_eq; simpl.
+    intros tr tr' Htr Htr'. unfold NIExists.ktr in *.
+    rewrite Htr in Htr'. apply pack_injective in Htr'.
+    subst tr. auto.
+
+    unfold vars_eq; simpl.
+    generalize (eval_hdlr_expr PAYD COMPT COMPS KSTD c m
+      (kst PAYD COMPT COMPS KSTD s) env e).
+    simpl in *. clear e. intros.
+    destruct s as [cs tr st].
+    clear H. destruct KSTD as [n kstd].
+    induction n.
+      auto.
+
+      destruct kstd. simpl in *.
+      destruct i.
+        match goal with
+        |- context [ if ?e then _ else _ ]
+          => destruct e
+        end; simpl in *.
+          f_equal. destruct st. simpl. apply IHn; auto.
+          rewrite <- vlblr_shift; auto.
+
+          f_equal. destruct st. simpl. apply IHn; auto.
+          rewrite <- vlblr_shift; auto.
+
+        unfold fin in *. rewrite Hvar. f_equal.
+Qed.
+
+Lemma stupd_high : forall c m envd i clblr vlblr llblr
+  (e:expr COMPT (hdlr_term (CT _ _ c) (CTAG _ m)) envd _) Hmatch,
+  vlblr i = false \/
+  hdlr_expr_ok_high _ _ _ _ e vlblr llblr = true ->
+  cmd_ok_high c m envd (StUpd (hdlr_term (CT _ _ c) (CTAG _ m)) envd i e)
+    clblr vlblr llblr Hmatch.
+Proof.
+  intros c m envd i clblr vlblr llblr e Hmatch H. destruct H as [Hlblr | Hexpr].
+    split.
+      unfold states_ok, high_out_eq in *. simpl. apply H1.
+
+      unfold states_ok, vars_eq in *; simpl.
+      generalize (eval_hdlr_expr PAYD COMPT COMPS KSTD c m
+        (kst PAYD COMPT COMPS KSTD s1) env1 e).
+      generalize (eval_hdlr_expr PAYD COMPT COMPS KSTD c m
+        (kst PAYD COMPT COMPS KSTD s2) env2 e).
+      simpl in *. clear e. intros.
+      destruct s1 as [cs1 tr1 st1].
+      destruct s2 as [cs2 tr2 st2].
+      clear H. clear H0. destruct KSTD as [n kstd].
+      induction n.
+        auto.
+
+        destruct kstd. simpl in *. destruct H1.
+        destruct i.
+        match goal with
+        |- context [ if ?e then _ else _ ]
+          => destruct e
+        end; simpl in *.
+        inversion H0. f_equal. destruct st1. destruct st2.
+        simpl. apply IHn; auto.
+        rewrite <- vlblr_shift; auto.
+        
+        inversion H0. f_equal. destruct st1. destruct st2.
+        simpl. apply IHn; auto.
+        rewrite <- vlblr_shift; auto.
+        
+        unfold fin in *. rewrite Hlblr in *.
+        inversion H0. simpl. f_equal. auto.
+        
+    split.
+
+      unfold states_ok, high_out_eq in *. simpl. apply H1.
+      
+      unfold vars_eq in *; simpl.
+      erewrite hdlr_expr_ok_high_correct
+        with (env1:=env1) (env2:=env2); eauto.
+      generalize (eval_hdlr_expr PAYD COMPT COMPS KSTD c m
+        (kst PAYD COMPT COMPS KSTD s2) env2 e).
+      destruct s1; destruct s2. simpl in *. clear Hexpr e.
+      simpl. destruct H1 as [Hout Hvars]. clear Hout.
+      clear H H0. destruct KSTD as [n kstd]. unfold vars_eq in *.
+      simpl in *. intros.
+      induction n.
+        auto.
+        
+        destruct kstd.
+        destruct i; simpl in *;
+          match goal with
+          |- context [if ?e then _ else _ ]
+            => destruct e
+          end; inversion Hvars; f_equal;
+          apply IHn; auto.
+Qed.
+
+Lemma stupd_high_all : forall c m envd i clblr vlblr llblr
+  (e:expr COMPT (hdlr_term (CT _ _ c) (CTAG _ m)) envd _) Hmatch,
+  vlblr i = false \/
+  hdlr_expr_ok_high _ _ _ _ e vlblr llblr = true ->
+  all_cmd_ok_high c m envd (StUpd (hdlr_term (CT _ _ c) (CTAG _ m)) envd i e)
+    clblr vlblr llblr Hmatch.
+Proof.
+  apply stupd_high.
+Qed.
+
+Fixpoint match_all_cfg_pat n : forall (vd:svec desc n),
+  shvec sdenote_desc_conc_pat vd :=
+  match n as _n return
+    forall (_vd:svec desc _n), shvec sdenote_desc_conc_pat _vd
+  with
+  | O => fun _ => tt
+  | S n' => fun vd =>
+    match vd with
+    | (vd0, vd') =>
+      (None, match_all_cfg_pat n' vd')
+    end
+  end.
+
+Definition match_all_pat ct :=
+  {| conc_pat_type:=ct
+    ; conc_pat_conf:=match_all_cfg_pat _
+    (projT2 (comp_conf_desc COMPT COMPS ct)) |}.
+
+Lemma match_all_pat_correct : forall ct c,
+  comp_type _ _ c = ct ->
+  match_comp (match_all_pat ct) c = true.
+Proof.
+  intros ct c Hct. unfold match_all_pat.
+  unfold match_comp, Reflex.match_comp, match_comp_pf.
+  destruct (COMPTDEC (comp_type COMPT COMPS c)
+           (conc_pat_type COMPT COMPS
+              {|
+              conc_pat_type := ct;
+              conc_pat_conf := match_all_cfg_pat
+                                 (projT1 (comp_conf_desc COMPT COMPS ct))
+                                 (projT2 (comp_conf_desc COMPT COMPS ct)) |})); try contradiction.
+  simpl in *. subst ct. rewrite UIP_refl with (p:=e).
+  destruct c. simpl in *. destruct (comp_conf_desc COMPT COMPS comp_type) as [n cfg].
+  induction n.
+    auto.
+
+    destruct cfg. destruct comp_conf. simpl in *. apply IHn.
+Qed.
+
+(*Lemma ct_comp_expr : forall c m envd st env ct
+  (ce:expr COMPT (hdlr_expr (comp_type _ _ c) (tag _ m)) envd (Comp _ ct)),
+  comp_type _ _ 
+  
+Lemma send_low : forall c m envd clblr vlblr ct
+  ce t ple,
+  clblr ct = None ->
+  cmd_ok_low c m envd (Send _ envd ct ce t ple) clblr vlblr.
+Proof.
+  intros c m envd clblr vlblr ct ce t ple Hnot_in.
+  unfold cmd_ok_low, states_ok. intros.
+  split.
+    unfold high_out_eq. intros. destruct s as [? [?] ?].
+    simpl in *. repeat uninhabit. simpl.
+expr COMPT
+         (Reflex.hdlr_term PAYD COMPT COMPS KSTD (CT COMPT COMPS c)
+            (CTAG PAYD m)) envd (Comp COMPT ct)
+(eval_hdlr_expr PAYD COMPT COMPS KSTD c m kst env ce)
+    destruct (eval_hdlr_expr PAYD COMPT COMPS KSTD c m kst env ce). auto.
+
+    unfold vars_eq. simpl. auto.
+Qed.*)
+
+Lemma send_low_ccomp : forall c m envd clblr vlblr t ple,
+  cmd_ok_low c m envd (Send _ envd _
+    (Term _ _ _ (CComp _ _ _ _ _ _ _)) t ple) clblr vlblr.
+Proof.
+  intros c m envd clblr vlblr t ple.
+  unfold cmd_ok_low, states_ok. intros.
+  split.
+    unfold high_out_eq. intros. destruct s as [? [?] ?].
+    simpl in *. repeat uninhabit. simpl. rewrite H0. auto.
+
+    unfold vars_eq. simpl. auto.
+Qed.
+
+Lemma send_high_all : forall c m envd clblr vlblr llblr ct
+  ce t ple Hmatch,
+  hdlr_expr_ok_high _ _ _ _ ce vlblr llblr = true ->
+  pl_expr_ok_high _ _ _ _ _ ple vlblr llblr = true ->
+  all_cmd_ok_high c m envd (Send _ envd ct ce t ple) clblr vlblr llblr Hmatch.
+Proof.
+  simpl. unfold cmd_ok_high. unfold states_ok. simpl.
+  intros c m envd clblr vlblr llblr ct ce t ple Hmatch Hexpr
+    Hpexpr env1 env2 s1 s2 i ? ? Hstates Hlocals.
+  split.
+    unfold high_out_eq. intros tr tr' Htr Htr'.
+    destruct s1 as [? [ ? ] ?]_eqn. destruct s2 as [? [ ? ] ?]_eqn. simpl in *.
+    repeat uninhabit. simpl. inversion Heqk. inversion Heqk0.
+    apply f_equal with (f:=Reflex.kst _ _ _ _) in Heqk.
+    apply f_equal with (f:=Reflex.kst _ _ _ _) in Heqk0.
+    simpl in *. rewrite <- Heqk. rewrite <- Heqk0.
+    destruct Hstates as [Hout Hvars]. unfold high_out_eq in Hout.
+    erewrite Hout; eauto.
+    erewrite hdlr_expr_ok_high_correct with (s2:=s2) (clblr:=clblr); eauto.
+    erewrite pl_hdlr_expr_ok_high_correct with (s2:=s2) (clblr:=clblr); eauto.
+    subst s1. subst s2. unfold states_ok. auto.
+    subst s1. subst s2. unfold states_ok. auto.
+
+    unfold vars_eq in *. simpl. apply Hstates.
+Qed.
+
+(*Lemma send_high_all_low_comp : forall c m envd clblr vlblr llblr ct
+  ce t ple,
+  ct_not_in_clblr ct clblr ->
+  all_cmd_ok_high c m envd (Send _ envd ct ce t ple) clblr vlblr llblr.
+Proof.
+  intros c m envd clblr vlblr llblr ct ce t ple Hnot_in.
+  simpl. unfold cmd_ok_high, states_ok. intros.
+  split.
+    unfold high_out_eq in *. intros. destruct s1 as [? [?] ?]; destruct s2 as [? [?] ?].
+    simpl in *. repeat uninhabit. simpl. repeat erewrite not_in_clblr; eauto.
+    destruct H0. auto.
+    destruct (eval_hdlr_expr PAYD COMPT COMPS KSTD c m kst0 env2 ce). auto.
+    destruct (eval_hdlr_expr PAYD COMPT COMPS KSTD c m kst env1 ce). auto.
+
+    unfold vars_eq. simpl. destruct H0. auto.
+Qed.
+*)
+
+Lemma call_low : forall c m envd clblr vlblr
+  e es i EQ,
+  cmd_ok_low c m envd (Call _ envd e es i EQ) clblr vlblr.
+Proof.
+  intros c m envd clblr vlblr e es i EQ.
+  simpl. unfold cmd_ok_low. intros.
+  unfold states_ok, high_out_eq, vars_eq in *. simpl.
+  split.
+    intros. destruct s as [? [?] ?].
+    simpl in *. repeat uninhabit. simpl. auto.
+
+    auto.
+Qed.
+
+Lemma call_high_all : forall c m envd clblr vlblr llblr
+  e es i EQ Hmatch,
+  all_cmd_ok_high c m envd (Call _ envd e es i EQ) clblr vlblr llblr Hmatch.
+Proof.
+  intros c m envd clblr vlblr llblr e es i EQ Hmatch.
+  simpl. unfold cmd_ok_high. intros.
+  unfold states_ok, high_out_eq, vars_eq in *. simpl.
+  split.
+    intros. destruct s1 as [? [?] ?]; destruct s2 as [? [?] ?].
+    simpl in *. repeat uninhabit. simpl. destruct H1. erewrite H1; eauto.
+
+    apply H1.
+Qed.
+
+Lemma spawn_high_all : forall c m envd clblr vlblr llblr ct
+  ple i EQ Hmatch,
+  pl_expr_ok_high _ _ _ _ _ ple vlblr llblr = true ->
+  all_cmd_ok_high c m envd (Spawn _ envd ct ple i EQ) clblr vlblr llblr Hmatch.
+Proof.
+  simpl. unfold cmd_ok_high. unfold states_ok. simpl.
+  intros c m envd clblr vlblr llblr ct ple i EQ Hmatch
+    Hpexpr env1 env2 s1 s2 f ? ? Hstates Hlocals.
+  split.
+    unfold high_out_eq. intros tr tr' Htr Htr'.
+    destruct s1 as [? [ ? ] ?]_eqn. destruct s2 as [? [ ? ] ?]_eqn. simpl in *.
+    repeat uninhabit. simpl. inversion Heqk. inversion Heqk0.
+    apply f_equal with (f:=Reflex.kst _ _ _ _) in Heqk.
+    apply f_equal with (f:=Reflex.kst _ _ _ _) in Heqk0.
+    simpl in *. rewrite <- Heqk. rewrite <- Heqk0.
+    destruct Hstates as [Hout Hvars]. unfold high_out_eq in Hout.
+    erewrite Hout; eauto.
+    erewrite pl_hdlr_expr_ok_high_correct with (s2:=s2) (clblr:=clblr); eauto.
+    subst s1. subst s2. unfold states_ok. auto.
+
+    unfold vars_eq in *. simpl. apply Hstates.
+Qed.
+
+Lemma ite_low : forall c m envd clblr vlblr
+  e cmd1 cmd2,
+  cmd_ok_low c m envd cmd1 clblr vlblr ->
+  cmd_ok_low c m envd cmd2 clblr vlblr ->
+  cmd_ok_low c m envd (Ite _ envd e cmd1 cmd2) clblr vlblr.
+Proof.
+  intros c m envd clblr vlblr e cmd1 cmd2 Hcmd1 Hcmd2.
+  unfold cmd_ok_low in *. intros env s i. simpl.
+  destruct (num_eq
+              (eval_hdlr_expr PAYD COMPT COMPS KSTD c m
+                 (kst PAYD COMPT COMPS KSTD s) env e) FALSE); auto.
+Qed.
+
+Lemma ite_high_all : forall c m envd clblr vlblr llblr
+  e cmd1 cmd2 Hmatch,
+  hdlr_expr_ok_high _ _ _ _ e vlblr llblr = true ->
+  all_cmd_ok_high c m envd cmd1 clblr vlblr llblr Hmatch ->
+  all_cmd_ok_high c m envd cmd2 clblr vlblr llblr Hmatch ->
+  all_cmd_ok_high c m envd (Ite _ envd e cmd1 cmd2) clblr vlblr llblr Hmatch.
+Proof.
+  intros c m envd clblr vlblr llblr e cmd1 cmd2 Hmatch Hexpr Hcmd1 Hcmd2.
+  simpl. rewrite Hexpr. auto.
+Qed.
+
+Lemma seq_low : forall clblr vlblr c m envd cmd1 cmd2,
+  cmd_ok_low c m envd cmd1 clblr vlblr ->
+  cmd_ok_low c m envd cmd2 clblr vlblr ->
+  cmd_ok_low c m envd (Seq _ _ cmd1 cmd2) clblr vlblr.
+Proof.
+  intros clblr vlblr c m envd cmd1 cmd2 Hcmd1 Hcmd2.
+  split.
+    unfold cmd_ok_low, high_out_eq, ve_st, kstate_run_prog in *. simpl in *.
+    intros. destruct i as [i1 i2]. specialize (Hcmd1 env s i1 H H0).
+    destruct Hcmd1 as [Hout1 ?].
+    destruct (hdlr_state_run_cmd PAYD COMPT COMPTDEC COMPS KSTD c m envd
+                  {| hdlr_kst := s; hdlr_env := env |} cmd1 i1) as [st env']_eqn.
+    assert (ReachInter st) as HRI.
+      apply f_equal with (f:=hdlr_kst _ _ _ _ _) in Heqh. simpl in Heqh.
+      subst st. eapply ReachInter_run; eauto.
+    specialize (Hcmd2 env' st i2 HRI H0). destruct Hcmd2 as [Hout2 ?].
+    destruct st as [? [tr''] ?]. simpl in *. rewrite Hout1 with (tr':=tr''); auto.
+    apply Hout2 with (tr:=tr'') (tr':=tr'); auto. rewrite <- Heqh. auto.
+
+    unfold cmd_ok_low, vars_eq, ve_st, kstate_run_prog in *. simpl in *.
+    destruct i as [i1 i2].
+    specialize (Hcmd1 env s i1 H H0). destruct Hcmd1 as [? Hvar1].
+    destruct (hdlr_state_run_cmd PAYD COMPT COMPTDEC COMPS KSTD c m envd
+                  {| hdlr_kst := s; hdlr_env := env |} cmd1 i1) as [st env']_eqn.
+    assert (ReachInter st) as HRI.
+      destruct s as [? [?] ?].
+      apply f_equal with (f:=hdlr_kst _ _ _ _ _) in Heqh. simpl in Heqh.
+      subst st. eapply ReachInter_run; eauto.
+    specialize (Hcmd2 env' st i2 HRI H0). destruct Hcmd2 as [? Hvar2].
+    rewrite Hvar1. simpl in *. rewrite Heqh. apply Hvar2.
+Qed.
+
+Lemma seq_high_all : forall c m envd cmd1 cmd2 clblr vlblr llblr Hmatch,
+  all_cmd_ok_high c m envd cmd1 clblr vlblr llblr Hmatch ->
+  all_cmd_ok_high c m envd cmd2 clblr vlblr
+    (get_llblr (CT _ _ c) (CTAG _ m) envd cmd1 (get_ccomp_cfgp c clblr Hmatch) clblr vlblr llblr) Hmatch ->
+  all_cmd_ok_high c m envd (Seq _ _ cmd1 cmd2) clblr vlblr llblr Hmatch.
+Proof.
+  simpl. auto.
+Qed.
+(*  intros c m envd cmd1 cmd2 clblr vlblr llblr Hcmd1 Hcmd2.
+    unfold cmd_ok_high, high_out_eq, ve_st, kstate_run_prog in *. simpl in *.
+    intros. destruct i as [i1 i2]. specialize (Hcmd1 env1 env2 s1 s2 i1 H H0).
+    simpl in *.
+    destruct (hdlr_state_run_cmd PAYD COMPT COMPTDEC COMPS KSTD c m envd
+                  {| hdlr_kst := s1; hdlr_env := env1 |} cmd1 i1) as [s1' env1']_eqn.
+    destruct (hdlr_state_run_cmd PAYD COMPT COMPTDEC COMPS KSTD c m envd
+                  {| hdlr_kst := s2; hdlr_env := env2 |} cmd1 i1) as [s2' env2']_eqn.
+    simpl in *.
+    apply Hcmd2; intuition.
+    apply f_equal with (f:=hdlr_env _ _ _ _ _) in Heqh.
+    apply f_equal with (f:=hdlr_env _ _ _ _ _) in Heqh0.
+    simpl in *. subst env1'. subst env2'.
+    eapply get_llblr_correct; eauto.
+Qed.*)
+
+Lemma high_out_eq_inter_ve_st : forall c m s tr clblr,
+  Reflex.ktr _ _ _ _ s = inhabits tr ->
+  high_out_eq _ _ _ _ s (mk_inter_ve_st PAYD COMPT COMPS KSTD c m s tr) clblr.
+Proof.
+  unfold high_out_eq, mk_inter_ve_st. simpl. intros.
+  remove_redundant_ktr. repeat uninhabit. auto.
+Qed.
+
+Lemma high_out_trans : forall (s1 s2 s3:kstate) clblr,
+  high_out_eq _ _ _ _ s1 s2 clblr ->
+  high_out_eq _ _ _ _ s2 s3 clblr ->
+  high_out_eq _ _ _ _ s1 s3 clblr.
+Proof.
+  intros. unfold high_out_eq in *.
+  intros. destruct s2. destruct ktr0.
+  rewrite <- H0 with (tr:=k) (tr':=tr'); auto.
+Qed.
+
+Lemma high_out_eq_refl : forall (s:kstate) clblr,
+  high_out_eq _ _ _ _ s s clblr.
+Proof.
+  intros. unfold high_out_eq. intros.
+  remove_redundant_ktr. auto.
+Qed.
+
+Lemma vars_eq_refl : forall (s:kstate) vlblr,
+  vars_eq _ _ _ _ s s vlblr.
+Proof.
+  auto.
+Qed.
+
+Lemma high_out_eq_sym : forall (s s':kstate) clblr,
+  high_out_eq _ _ _ _ s s' clblr ->
+  high_out_eq _ _ _ _ s' s clblr.
+Proof.
+  unfold high_out_eq. intros.
+  symmetry. auto.
+Qed.
+
+Lemma vars_eq_sym : forall (s s':kstate) vlblr,
+  vars_eq _ _ _ _ s s' vlblr ->
+  vars_eq _ _ _ _ s' s vlblr.
+Proof.
+  unfold vars_eq. intros. auto.
+Qed.
+
+Lemma vars_eq_inter_ve_st : forall c m s tr clblr,
+  Reflex.ktr _ _ _ _ s = inhabits tr ->
+  vars_eq _ _ _ _ s (mk_inter_ve_st PAYD COMPT COMPS KSTD c m s tr) clblr.
+Proof.
+  auto.
+Qed.
+
+Lemma vars_eq_trans : forall (s1 s2 s3:kstate) clblr,
+  vars_eq _ _ _ _ s1 s2 clblr ->
+  vars_eq _ _ _ _ s2 s3 clblr ->
+  vars_eq _ _ _ _ s1 s3 clblr.
+Proof.
+  intros. unfold vars_eq in *. etransitivity; eauto.
+Qed.
+
+Lemma nop_low : forall clblr vlblr c m envd,
+  cmd_ok_low c m envd (Nop _ _) clblr vlblr.
+Proof.
+  intros clblr vlblr c m envd.
+  unfold cmd_ok_low, states_ok. intros env s.
+  simpl. split.
+    apply high_out_eq_refl.
+    apply vars_eq_refl.
+Qed.
+
+Lemma nop_high : forall clblr vlblr c m envd llblr Hmatch,
+  cmd_ok_high c m envd (Nop _ _) clblr vlblr llblr Hmatch.
+Proof.
+  intros clblr vlblr c m envd llblr.
+  unfold cmd_ok_high, states_ok. intros.
+  simpl. auto.
+Qed.
+
+Lemma nop_high_all : forall clblr vlblr c m envd llblr Hmatch,
+  all_cmd_ok_high c m envd (Nop _ _) clblr vlblr llblr Hmatch.
+Proof.
+  apply nop_high.
+Qed.
+
+Section WITH_HANDLERS_INIT.
+
+Variable HANDLERS : handlers PAYD COMPT COMPS KSTD.
+Variable INIT : init_prog PAYD COMPT COMPS KSTD IENVD.
+Definition ValidExchange := Reflex.ValidExchange PAYD COMPT COMPTDEC COMPS KSTD HANDLERS.
 
 Lemma prune_nop_1 : forall clblr vlblr c m i s s',
   ValidExchange c m i s s' ->
@@ -81,40 +1996,83 @@ Proof.
       unfold vars_eq. simpl. auto.
 Qed.
 
-(*
-Print high_ok.
-Print kstate_run_prog.
-Print high_out_eq.
-Print mk_inter_ve_st.
-Lemma skip_ve : forall clblr vlblr c m i s1 s1' s2 s2',
-  high_out_eq PAYD COMPT COMPS KSTD s1 s2 clblr ->
-  vars_eq PAYD COMPT COMPS KSTD s1 s2 vlblr ->
-  Reflex.ValidExchange PAYD COMPT COMPTDEC COMPS KSTD HANDLERS c m i s1 s1' ->
-  Reflex.ValidExchange PAYD COMPT COMPTDEC COMPS KSTD HANDLERS c m i s2 s2' ->
-  (forall tr1 tr1' tr2 tr2',
-    ktr _ _ _ _ s1 = inhabits tr1 ->
-    ktr _ _ _ _ s1' = inhabits tr1' ->
-    ktr _ _ _ _ s2 = inhabits tr2 ->
-    ktr _ _ _ _ s2' = inhabits tr2' ->
-    vars_eq PAYD COMPT COMPS KSTD s1 s2 vlblr ->
-    high_out_eq PAYD COMPT COMPS KSTD
-      (hdlr_kst _ _ _ _ _ (hdlr_state_run_cmd PAYD COMPT COMPTDEC COMPS KSTD c m
-        (projT1 (HANDLERS (tag _ m) (comp_type _ _ c)))
-        (default_hdlr_state PAYD COMPT COMPS KSTD (mk_inter_ve_st _ _ _ _ c m s1 tr1)
-          (projT1 (HANDLERS (tag _ m) (comp_type _ _ c))))
-        (projT2 (HANDLERS (tag _ m) (comp_type _ _ c))) i))
-      (hdlr_kst _ _ _ _ _ (hdlr_state_run_cmd PAYD COMPT COMPTDEC COMPS KSTD c m
-        (projT1 (HANDLERS (tag _ m) (comp_type _ _ c)))
-        (default_hdlr_state PAYD COMPT COMPS KSTD (mk_inter_ve_st _ _ _ _ c m s2 tr1)
-          (projT1 (HANDLERS (tag _ m) (comp_type _ _ c))))
-        (projT2 (HANDLERS (tag _ m) (comp_type _ _ c))) i)) clblr)->
-  high_out_eq PAYD COMPT COMPS KSTD s1' s2' clblr.
+Definition low_ok'' clblr vlblr := forall c m,
+  lblr_match_comp COMPT COMPTDEC COMPS clblr c = false ->
+  cmd_ok_low c m (projT1 (HANDLERS (tag PAYD m) (comp_type COMPT COMPS c)))
+    (projT2 (HANDLERS (tag PAYD m) (comp_type COMPT COMPS c))) clblr vlblr.
+
+Definition high_ok'' clblr vlblr :=
+  forall c m
+    (Hmatch:lblr_match_comp COMPT COMPTDEC COMPS clblr c = true),
+    cmd_ok_high c m (projT1 (HANDLERS (tag PAYD m) (comp_type COMPT COMPS c)))
+    (projT2 (HANDLERS (tag PAYD m) (comp_type COMPT COMPS c)))
+    clblr vlblr (fun _ => true) Hmatch.
+
+Definition high_ok_all clblr vlblr :=
+  forall c m
+    (Hmatch:lblr_match_comp COMPT COMPTDEC COMPS clblr c = true),
+    all_cmd_ok_high c m (projT1 (HANDLERS (tag PAYD m) (comp_type COMPT COMPS c)))
+    (projT2 (HANDLERS (tag PAYD m) (comp_type COMPT COMPS c)))
+    clblr vlblr (fun _ => true) Hmatch.
+
+Lemma Reach_ReachInter : forall s,
+  Reach PAYD COMPT COMPTDEC COMPS IENVD KSTD INIT HANDLERS s -> ReachInter s.
 Proof.
-  intros clblr vlblr c m i s1 s1' s2 s2' Hout Hvars Hve1 Hve2 Hunfolded.
-  inversion Hve1. inversion Hve2. clear Hve1. clear Hve2.
-    subst s'0. subst s'. unfold hdlrs. unfold hdlrs0.
-    unfold kstate_run_prog. unfold hdlr_state_run_cmd.
-        
-*)
+  intros s HReach.
+  induction HReach.
+    inversion H. subst s0. repeat econstructor.
+
+    inversion H. subst s'0. unfold mk_inter_ve_st.
+    repeat econstructor; auto.
+
+    inversion H. unfold mk_bogus_st. repeat econstructor; auto.
+Qed.
+
+Theorem ni_suf'' : forall clblr vlblr,
+  low_ok'' clblr vlblr ->
+  high_ok'' clblr vlblr ->
+  NI PAYD COMPT COMPTDEC COMPS
+  IENVD KSTD INIT HANDLERS clblr vlblr.
+Proof.
+  intros. apply ni_suf'.
+  unfold low_ok', low_ok'', cmd_ok_low, states_ok, ve_st in *.
+  intros.
+  split.
+    apply high_out_trans with (s2:=mk_inter_ve_st PAYD COMPT COMPS KSTD c m s tr); auto.
+    apply high_out_eq_inter_ve_st; auto.
+    apply H; auto. unfold mk_inter_ve_st. repeat econstructor; auto. apply Reach_ReachInter; auto.
+    apply vars_eq_trans with (s2:=mk_inter_ve_st PAYD COMPT COMPS KSTD c m s tr); auto.
+    apply H; auto. unfold mk_inter_ve_st. repeat econstructor; auto. apply Reach_ReachInter; auto.
+
+  unfold high_ok', high_ok'', cmd_ok_high, states_ok, ve_st in *.
+  intros. apply H0; auto. 
+  unfold mk_inter_ve_st. repeat econstructor; auto. apply Reach_ReachInter; auto.
+  unfold mk_inter_ve_st. repeat econstructor; auto. apply Reach_ReachInter; auto.
+  split.
+    apply high_out_trans with (s2:=s1). apply high_out_eq_sym.
+    apply high_out_eq_inter_ve_st; auto.
+    apply high_out_eq_sym. apply high_out_trans with (s2:=s2).
+    apply high_out_eq_sym. apply high_out_eq_inter_ve_st; auto.
+    apply high_out_eq_sym; auto.
+
+    apply vars_eq_trans with (s2:=s1). apply vars_eq_sym.
+    apply vars_eq_inter_ve_st; auto.
+    apply vars_eq_sym. apply vars_eq_trans with (s2:=s2).
+    apply vars_eq_sym. apply vars_eq_inter_ve_st; auto.
+    apply vars_eq_sym; auto.
+Qed.
+
+Theorem ni_suf_all : forall clblr vlblr,
+  low_ok'' clblr vlblr ->
+  high_ok_all clblr vlblr ->
+  NI PAYD COMPT COMPTDEC COMPS
+  IENVD KSTD INIT HANDLERS clblr vlblr.
+Proof.
+  intros. apply ni_suf''; auto.
+    unfold high_ok''. intros. apply cmd_ok_high'_ok.
+    apply all_cmd_ok_high_correct; auto.
+Qed.
+
+End WITH_HANDLERS_INIT.
 
 End Prune.
