reflex/coq/Reflex.v
@@ -969,9 +969,9 @@ Inductive cmd : vcdesc -> Type :=
 | Call : forall (envd : vcdesc), expr envd (Desc str_d) -> list (expr envd (Desc str_d)) ->
     forall (i : fin (projT1 envd)), svec_ith (projT2 envd) i = Desc fd_d -> cmd envd
 | StUpd : forall envd i, expr envd (svec_ith (projT2 KSTD) i) -> cmd envd
-| CompLkup : forall (envd : vcdesc) cp,
-  cmd (existT _ (S (projT1 envd)) (svec_shift (Comp (comp_pat_type envd cp)) (projT2 envd))) ->
-  cmd envd -> cmd envd
+| CompLkup : forall (envd : vcdesc) cp (i : fin (projT1 envd)),
+  svec_ith (projT2 envd) i = Comp (comp_pat_type envd cp) ->
+  cmd envd -> cmd envd -> cmd envd
 .
 
 Record init_state (envd : vcdesc) :=
@@ -1072,7 +1072,7 @@ Fixpoint run_cmd_it {envd : vcdesc} {term} (cmd : cmd term envd) : InputTreeType
                            (run_cmd_it c2)
   | Ite _ _ c1 c2 => Comb (run_cmd_it c1)
                              (run_cmd_it c2)
-  | CompLkup _ _ c1 c2 => Comb (run_cmd_it c1)
+  | CompLkup _ _ _ _ c1 c2 => Comb (run_cmd_it c1)
                                (run_cmd_it c2)
   | _ => Unit
   end.
@@ -1148,8 +1148,20 @@ Fixpoint init_state_run_cmd (envd : vcdesc) (s : init_state envd) (cmd : cmd bas
      ; init_kst   := shvec_replace_ith _ _ (init_kst _ s) i v
      |}
 
-  | CompLkup envd cp c1 c2 => fun s i =>
+  | CompLkup envd cp i EQ c1 c2 => fun s i =>
     let ocdp := find_comp (eval_base_comp_pat _ (init_env _ s) cp) (init_comps _ s) in
+    match ocdp with
+    | Some cdp =>
+      let s' :=
+        {| init_comps := init_comps _ s
+         ; init_ktr   := init_ktr _ s
+         ; init_env   := shvec_replace_cast EQ (init_env _ s) cdp
+         ; init_kst   := init_kst _ s
+         |} in
+      init_state_run_cmd envd s' c1 (fst i)
+    | None => init_state_run_cmd envd s c2 (snd i)
+    end
+(*    let ocdp := find_comp (eval_base_comp_pat _ (init_env _ s) cp) (init_comps _ s) in
     match ocdp with
     | Some cdp =>
       let c := projT1 cdp in
@@ -1166,7 +1178,7 @@ Fixpoint init_state_run_cmd (envd : vcdesc) (s : init_state envd) (cmd : cmd bas
        ; init_kst   := init_kst _ s''
        |}
     | None   =>  init_state_run_cmd envd s c2 (snd i)
-    end
+    end*)
 
   end s input.
 
@@ -1247,8 +1259,23 @@ Fixpoint hdlr_state_run_cmd (envd : vcdesc) (s : hdlr_state envd) (cmd : cmd (hd
      ; hdlr_env := env
      |}
 
-  | CompLkup envd cp c1 c2 => fun s i =>
+  | CompLkup envd cp i EQ c1 c2 => fun s i =>
     let (s', env) := s in
+    let ocdp := find_comp (eval_hdlr_comp_pat (kst s') _ env cp) (kcs s') in
+    match ocdp with
+    | Some cdp =>
+      let s'' :=
+        {| hdlr_kst :=
+          {| kcs := kcs s'
+           ; ktr := ktr s'
+           ; kst := kst s'
+           |}
+         ; hdlr_env := shvec_replace_cast EQ env cdp
+         |} in
+      hdlr_state_run_cmd envd s'' c1 (fst i)
+    | None   =>  hdlr_state_run_cmd envd s c2 (snd i)
+    end
+(*    let (s', env) := s in
     let ocdp := find_comp (eval_hdlr_comp_pat (kst s') _ env cp) (kcs s') in
     match ocdp with
     | Some cdp =>
@@ -1272,7 +1299,7 @@ Fixpoint hdlr_state_run_cmd (envd : vcdesc) (s : hdlr_state envd) (cmd : cmd (hd
        ; hdlr_env := shvec_unshift cdesc sdenote_cdesc (projT1 envd) d (projT2 envd) (hdlr_env _ s'')
        |}
     | None   =>  hdlr_state_run_cmd envd s c2 (snd i)
-    end
+    end*)
   end s input.
 
 Fixpoint default_input {envd term} (c : cmd term envd) : s[[run_cmd_it c]] :=
@@ -1281,7 +1308,7 @@ Fixpoint default_input {envd term} (c : cmd term envd) : s[[run_cmd_it c]] :=
   | Call _ _ _ _ _ => devnull
   | Seq _ c1 c2 => (default_input c1, default_input c2)
   | Ite _ _ c1 c2 => (default_input c1, default_input c2)
-  | CompLkup _ _ c1 c2 => (default_input c1, default_input c2)
+  | CompLkup _ _ _ _ c1 c2 => (default_input c1, default_input c2)
   | _ => tt
   end.
 
@@ -2026,17 +2053,17 @@ Proof.
 Qed.
 
 Lemma vcdesc_fds_set_replace_comp : forall ct envd i
-  (EQ:svec_ith (projT2 envd) i = Comp ct) e c_fd cfg fds,
+  (EQ:svec_ith (projT2 envd) i = Comp ct) e c_fd cfg fds EQct,
   vdesc_fds_all_in cfg fds ->
   vcdesc_fds_all_in e fds ->
   vcdesc_fds_all_in (vd:=envd)
       (shvec_replace_cast EQ e
         (existT (fun c1 : comp => comp_type c1 = ct) 
           {|comp_type:=ct; comp_fd:=c_fd; comp_conf:=cfg|}
-          (Logic.eq_refl ct)))
+          EQct))
     (c_fd :: fds).
 Proof.
-  intros ct envd i EQ e c_fd cfg fds Hcfg_in Hall_in.
+  intros ct envd i EQ e c_fd cfg fds EQct Hcfg_in Hall_in.
   unfold vcdesc_fds_all_in, in_if_fd_cdesc. intro i'.
   pose proof (fin_eq_dec i i') as Hfeq_dec.
   destruct Hfeq_dec as [Hfeq | Hfneq].
@@ -2416,7 +2443,7 @@ Proof.
     | StUpd _ i ve => fun s =>
       let case := "StUpd _ i ve"%string in _
 
-    | CompLkup envd cp c1 c2 => fun s =>
+    | CompLkup envd cp i EQ c1 c2 => fun s =>
       let case := "CompLkup envd cp c1 c2"%string in _
 
     end s0
@@ -2512,7 +2539,25 @@ pose (ocdp := find_comp (eval_base_comp_pat _ e cp) cs).
 destruct ocdp as [ cdp | ]_eqn.
 (*Component found*)
 refine (
-  let c := projT1 cdp in
+ let s' :=
+        {| init_comps := init_comps _ s
+         ; init_ktr   := init_ktr _ s
+         ; init_env   := shvec_replace_cast EQ (init_env _ s) cdp
+         ; init_kst   := init_kst _ s
+         |} in
+  s'' <- self envd c1 s';
+  {{ Return s''}}
+); sep unfoldr simplr_base.
+unfold vcdesc_fds_all_in. intro i'. unfold in_if_fd_cdesc.
+destruct (fin_eq_dec i i'). subst i.
+rewrite shvec_ith_replace_cast_ith. rewrite EQ.
+pose proof (find_comp_suc envd e cp cs cdp Heqo).
+sep unfoldr simplr_base.
+rewrite shvec_ith_replace_cast_other; auto.
+unfold vcdesc_fds_all_in, in_if_fd_cdesc in *.
+apply H0; auto.
+
+(*  let c := projT1 cdp in
   let d := Comp (comp_pat_type _ _ cp) in
   let new_envd := (existT _ (S (projT1 envd)) (svec_shift d (projT2 envd))) in
   let s' := Build_init_state new_envd cs tr
@@ -2528,6 +2573,7 @@ refine (
   }}
 ); sep unfoldr simplr_base.
 unfold c; apply H; eapply find_comp_suc with (c:=cdp); eauto.
+*)
 
 (*Component not found*)
 refine (
@@ -2689,7 +2735,7 @@ Proof.
   | StUpd _ i ve => fun s =>
     let case := "StUpd _ i ve"%string in _
 
-  | CompLkup _ cp c1 c2 => fun s =>
+  | CompLkup _ cp i EQ c1 c2 => fun s =>
     let case := "CompLkup _ cp c1 c2"%string in _
 
   end s0
@@ -2799,6 +2845,27 @@ pose (ocdp := find_comp (eval_hdlr_comp_pat cc cm st envd env cp) cs).
 destruct ocdp as [ cdp | ]_eqn.
 (*Component found*)
 refine (
+  let s' :=
+    {| hdlr_kst :=
+      {| kcs := cs
+       ; ktr := tr
+       ; kst := st
+       |}
+     ; hdlr_env := shvec_replace_cast EQ env cdp
+     |} in
+  s'' <- self envd c1 s';
+  {{ Return s'' }}
+); sep unfoldr simplr_base.
+unfold vcdesc_fds_all_in. intro i'. unfold in_if_fd_cdesc.
+destruct (fin_eq_dec i i'). subst i.
+rewrite shvec_ith_replace_cast_ith. rewrite EQ.
+pose proof (find_comp_suc_hdlr cc cm envd env st cp cs cdp Heqo).
+sep unfoldr simplr_base.
+rewrite shvec_ith_replace_cast_other; auto.
+unfold vcdesc_fds_all_in, in_if_fd_cdesc in *.
+apply H1; auto.
+
+(*
   let c := projT1 cdp in
   let d := Comp (comp_pat_type _ _ cp) in
   let new_envd := (existT _ (S (projT1 envd)) (svec_shift d (projT2 envd))) in
@@ -2821,6 +2888,7 @@ refine (
   }}
 ); sep unfoldr simplr_base.
 apply H0. unfold c0; eapply find_comp_suc_hdlr with (c:=cdp); eauto.
+*)
 
 (*Component not found*)
 refine (
